cleans up lots of stuff, permits calls to Examples via X

Main.dfy
@@ -1,13 +1,27 @@
 include "Klon-HighLine.dfy"
 
+include "Example.dfy"
 
 include "Ownership-Recursive.dfy"
 include "Printing.dfy"
-
-//  include "Z2.dfy" // birmnamwood14, isownedby  - fast
-include "SSO.dfy"
+include "Graphing.dfy"
 
 
+//try this:
+  //time lately run Main.dfy c OF "" "{ rank=min; 3; } {rank=same; 2;} {rank=same; 1;} {rank=max; 0; 00;} { rank=same; i; j}  rankdir="TB"; margin=0; "  --allow-warnings --no-verify | tee DUMP.txt
+//then thid
+//csplit DUMP.txt %//STARTGRAPH%; mv xx00  test.gv ; dpdf test.gv ; open test.gv.pdf
+//
+//should take out both SSO and split
+// include "SSO.dfy" // ..ARGH!!
+//
+// datatype Split = Split(within : OWNR, without : OWNR, m : Klon)
+//
+// function split(oo : OWNR, m : Klon) : Split
+//   requires forall o <- oo :: m.objectReadyInKlown(o)
+// {
+//   Split( (set o <- oo | inside(o, m.o)), (set o <- oo | outside(o, m.o)), m)
+// }
 
 
 
@@ -15,144 +29,37 @@ const protoTypes : map<string, Mode> := fields({"t","a","b","c","d","e","k","l",
   // map["fa":= Evil]["fb":=Evil]  //wrong but will likely do for now?
 
 
-datatype Split = Split(within : OWNR, without : OWNR, m : Klon)
-
-function split(oo : OWNR, m : Klon) : Split
-  requires forall o <- oo :: m.objectReadyInKlown(o)
-{
-  Split( (set o <- oo | inside(o, m.o)), (set o <- oo | outside(o, m.o)), m)
-}
-
-
-lemma {:verify false} objectReadyToOwnerReadyInKlon(o : Object, m : Klon)
-  requires m.ownersReadyInKlown(o) || m.objectReadyInKlown(o)
-   ensures forall oo <- o.AMFX :: oo.Ready()
-   ensures forall oo <- o.AMFX :: oo.AMFO <= m.m.Keys
-   ensures forall oo <- o.AMFX :: m.objectReadyInKlown(oo)
-  {
-    o.ExtraReady();
-  }
-
-function map2vmap(m : map<Object,Object>) : vmap<Object,Object>
-  requires AllMapEntriesAreUnique(m)
-  { m }
 
 
 
-function  sporamfo(o : Object) : Owner {(set oo : Object <- o.owner, ooo : Object <- oo.AMFO :: ooo) + {o}}
-  //takes an object via it's owners to its AMFO
-function sporamfx(o : Object) : Owner {set oo : Object <- o.owner,   ooo : Object <- oo.AMFO :: ooo}
-  //takes an object via it's owners to its AMFX
-function sporamfb(o : Object) : Owner {set oo : Object <- o.bound,   ooo : Object <- oo.AMFO :: ooo}
-  //takes an object via it's owners to its AMFB
-function splatten(os : Owner) : Owner {(set oo : Object <- os,       ooo : Object <- oo.AMFO :: ooo)}
-  //takes an Owner via it's owners to its AMFO
 
 
-function sporrel(k : Object, m : Klon) : string
-  requires k.Ready()
- {
-   if (k == m.o) then ("pivot  ")
-     else if (outside(k, m.o))
-       then ("outside")
-       else ("inside ")
- }
-
-
-datatype PrintOptions = PrintOptions (
-  graph : string,
-  lines : string,
-  nodes : string,
-  extra : string
-)
-{
-  predicate lineOpt(c : char)   { (lines == "") || (c in lines) }
-  predicate nodeOpt(n : string) { (nodes == "") || (n == "") || (n[0] in nodes) }
-}
-
-
-method getPrintOptions(args : seq<string>) returns (pops : PrintOptions)
-{
-  var ALLLINEOPTS := "OoBbFMR";
-  var aa := args;
-  if (|args| < 2)
-     { print "got no arguments!!\n";
-       print "going with dahlia 9 _" + ALLLINEOPTS + " _c _extra...\n";
-       aa := ["dahlia", "9"];
-       }
-
-   var graph : string := "";
-   var lines : string := "";
-   var nodes : string := "";
-   var extra : string := "";
-
-   if (|aa| > 1) { graph := aa[1]; }
-   if (|aa| > 2) { lines := aa[2]; }
-   if (|aa| > 3) { nodes := aa[3]; }
-   if (|aa| > 4) { extra := aa[4]; }
-
-   print "graph = ", graph, "\n";
-   print "lines = ", lines, "\n";
-   print "nodes = ", nodes, "\n";
-   print "extra = ", extra, "\n";
-
-   pops := PrintOptions(graph, lines, nodes, extra);
-
-   print "ALLLINEOPTS:\n";
-   for x := 0 to |ALLLINEOPTS| {
-       var opt : char := ALLLINEOPTS[x];
-       print opt, " ", pops.lineOpt(opt), "\n";
-   }
-
-}
 
 method {:verify false} Main(args : seq<string>)
 {
   print "Snick! Snack! Snock!\n";
 
-  var pops := getPrintOptions(args);
-
+  var gops := getGraphOptions(args);
 
   var t,a,b,c,d,e,k,l,m,os,oq, loutName := zandal0();
 
- if (pops.graph == "0")
-    {
-      t,a,b,c,d,e,k,l,m,os,oq, loutName := zandal10();
-    }
+ if (gops.graph == "7") { t,a,b,c,d,e,k,l,m,os,oq, loutName := wrangle7(); }
+ if (gops.graph == "8") { t,a,b,c,d,e,k,l,m,os,oq, loutName := jandal8(); }
+ if (gops.graph == "s") { t,a,b,c,d,e,k,l,m,os,oq, loutName := sandal8(); }
+ if (gops.graph == "r") { t,a,b,c,d,e,k,l,m,os,oq, loutName := randal9(); }
 
- if (pops.graph == "9")
-    {
-      t,a,b,c,d,e,k,l,m,os,oq, loutName := zandal9();
-    }
+ if (gops.graph == "9") { t,a,b,c,d,e,k,l,m,os,oq, loutName := zandal9(); }
+ if (gops.graph == "b") { t,a,b,c,d,e,k,l,m,os,oq, loutName := zandal9bounded(); }
+ if (gops.graph == "c") { t,a,b,c,d,e,k,l,m,os,oq, loutName := zandal9capsul(); }
+ if (gops.graph == "d") { t,a,b,c,d,e,k,l,m,os,oq, loutName := zandal9tapsul(); }
 
- if (pops.graph == "b")
-    {
-      t,a,b,c,d,e,k,l,m,os,oq, loutName := zandal9bounded();
-    }
+ if (gops.graph == "0") { t,a,b,c,d,e,k,l,m,os,oq, loutName := zandal10(); }
+ if (gops.graph == "1") { t,a,b,c,d,e,k,l,m,os,oq, loutName := zandal11(); }
+ if (gops.graph == "l") { t,a,b,c,d,e,k,l,m,os,oq, loutName := zandalList(); }
+ if (gops.graph == "t") { t,a,b,c,d,e,k,l,m,os,oq, loutName := zandalThreads(); }
 
- if (pops.graph == "l")
-    {
-      t,a,b,c,d,e,k,l,m,os,oq, loutName := zandalList();
-    }
+ if (gops.graph == "X") { print "launch\n"; ExampleMain(args[1..]); return; }
 
-
- if (pops.graph == "t")
-    {
-      t,a,b,c,d,e,k,l,m,os,oq, loutName := zandalThreads();
-    }
-
-
-
-
-//KLON fields
-  // m : vmap<Object,Object>,    //the  klon map
-  // o : Object,                 //object being copied
-  // clowner : Owner,            //owner of the clone
-  // clbound : Owner,            //bound of the clone
-  // oHeap : set<Object>,        //heap
-  // o_amfx : Owner,             //was o. so the AMFX of o
-  // //  c_amfb : OWNR,              //epected flattened bound of the clone..
-  // c_amfx : Owner
 
 
   var v : map<Object,Object> := map[
@@ -209,13 +116,13 @@ method {:verify false} Main(args : seq<string>)
   print "   layers=\"mapping:fields:owner:bound:amfo:bg\";\n";
 //  print "   concentrate=true;\n";
   print "   node [shape=box]\n\n";
-  print "//===\n", pops.extra,"\n//===\n";
+  print "//===\n", gops.extra,"\n//===\n";
 
-        graphobjectset(hs, km, pops);
+        graphobjectset(hs, km, gops);
 
-        if (pops.lineOpt('M')) { graphmapping(km.m, pops); }
+        if (gops.lineOpt('M')) { graphmapping(km.m, gops); }
 
-        if (pops.lineOpt('R')) {    graphrefs(hq, pops); }
+        if (gops.lineOpt('R')) {    graphrefs(hq, gops); }
 
 
  print "}\n\n\n";
@@ -229,994 +136,10 @@ method {:verify false} Main(args : seq<string>)
 
 }
 
- method {:verify false} do_object(o : Object, m : Klon)
-   requires m.objectReadyInKlown(o)
-   requires HighCalidFragilistic(m)
- {
-   var spl := split(o.AMFO, m);  //WARNING WILL ROBINSON!!!
-   print o.nick;
-   print "  AMFO=", ffmtnickset(o.AMFO);
-   print "  within=", ffmtnickset(spl.within);
-   print "  without=", ffmtnickset(spl.without);
 
-   if (spl.within == {})
-     { print " (only outside, skipping)\n"; return; }
-    else { nl(); }
 
-    print "   processing..\n";
-    print "   within " + o.nick, "  AMFO=", ffmtnickset(o.AMFO), "\n";
 
-    var trimmed := o.AMFO - m.o.AMFO;
-    print "   trimmed ", ffmtnickset(trimmed), "\n";
-
-    var translated : SSO := {};
-
-    while trimmed != {}
-    {
-       var y: Object;
-       y :| y in trimmed;
-       trimmed := trimmed - {y};
-
-       print "      ", y.nick,"  AMFO=", ffmtnickset(y.AMFO);
-       if (y.AMFO >= m.o.AMFO)
-         {
-            var trans : Owner := mapThruKlon( (y.AMFO - m.o.AMFO), m ) +  ( m.m[m.o].AMFO );
-            translated := translated + {trans};
-            print "  tr=",ffmtnickset(trans),"\n";
-         } else {
-            translated := translated + {y.AMFO};  print "        (outside)\n";
-         }
-
-    }
-
-    var reconnected := translated + obj2sso( m.m[m.o] );
-    print "   done " + o.nick, " translated AMFO=", ffmtsso(reconnected),     "\n";
-    print "        " + o.nick, " direct     AMFO=", ffmtsso(obj2sso(m.m[o])), "\n";
- }
-
-
-
- method {:verify false}  do_object_mod(o : Object, m : Klon)
-   requires m.objectReadyInKlown(o)
-   requires HighCalidFragilistic(m)
- {
-   var spl := split(o.AMFO, m);  //WARNING WILL ROBINSON!!!
-   print o.nick;
-   print "  AMFO=", ffmtnickset(o.AMFO);
-   print "  within=", ffmtnickset(spl.within);
-   print "  without=", ffmtnickset(spl.without);
-
-   if (spl.within == {})
-     { print " (only outside, skipping)\n"; return; }
-    else { nl(); }
-
-    print "   processing..\n";
-    print "   within " + o.nick, "  AMFO=", ffmtnickset(o.AMFO), "\n";
-
-    var trimmed := o.AMFO - m.o.AMFO;
-    print "   trimmed ", ffmtnickset(trimmed), "\n";
-
-    var translated : SSO := set y <- trimmed ::
-
-       if (y.AMFO >= m.o.AMFO) then
-         (
-            var trans : Owner := mapThruKlon( (y.AMFO - m.o.AMFO), m ) +  ( m.m[m.o].AMFO );
-            trans
-          ) else ( y.AMFO );
-
-    var reconnected := translated + obj2sso( m.m[m.o] );
-
-    print "   done " + o.nick, " translated AMFO=", ffmtsso(reconnected),     "\n";
-    print "        " + o.nick, " direct     AMFO=", ffmtsso(obj2sso(m.m[o])), "\n";
- }
-
-
-
- method {:verify false}  do_object_mod2(o : Object, m : Klon)
-   requires m.objectReadyInKlown(o)
-   requires HighCalidFragilistic(m)
- {
-   var spl := split(o.AMFO, m);  //WARNING WILL ROBINSON!!!
-   print o.nick;
-   print "  AMFO=", ffmtnickset(o.AMFO);
-   print "  within=", ffmtnickset(spl.within);
-   print "  without=", ffmtnickset(spl.without);
-
-   if ((set x <- o.AMFO | inside(x, m.o)) == {})
-     { print " (only outside, skipping)\n"; return; }
-    else { nl(); }
-
-    print "   processing..\n";
-    print "   within " + o.nick, "  AMFO=", ffmtnickset(o.AMFO), "\n";
-
-    var trimmed := o.AMFO - m.o.AMFO;
-    print "   trimmed ", ffmtnickset(trimmed), "\n";
-
-    var translated : SSO := ( set y <- trimmed ::
-
-       if (y.AMFO >= m.o.AMFO) then
-         (mapThruKlon( (y.AMFO - m.o.AMFO), m ) +  ( m.m[m.o].AMFO )
-         ) else ( y.AMFO ) )
-    ;
-
-    var reconnected := translated + obj2sso( m.m[m.o] );
-
-    print "   done " + o.nick, " translated AMFO=", ffmtsso(reconnected),     "\n";
-    print "        " + o.nick, " direct     AMFO=", ffmtsso(obj2sso(m.m[o])), "\n";
- }
-
-
-
-
- method {:verify false} do_object_mod3(o : Object, m : Klon)
-   requires m.objectReadyInKlown(o)
-   requires HighCalidFragilistic(m)
-   requires m.SuperCalidFragilistic()
-    ensures m.Calid()   //no fucking idea wwhy this is failing,  but qutie curious!
-    ensures m.AllLinesCalid()
- {
-   assert m.Calid();
-   assert m.AllLinesCalid();
-   var spl := split(o.AMFO, m);  //WARNING WILL ROBINSON!!!
-   print "o=",o.nick,"    m.o=", ffmtnickset(m.o.AMFO), "\n";
-
-   print "\n\n           AMFO=", ffmtnickset(o.AMFO);
-   print "\n           within=", ffmtnickset(spl.within);
-   print "\n          without=", ffmtnickset(spl.without);
-   print "\no.AMFO-m.o.AMFO**=", ffmtnickset(o.AMFO - m.o.AMFO);
-   print "\no.AMFO - {m.o}***=", ffmtnickset(o.AMFO - {m.o});
-   print "\no.AMFO -without  =", ffmtnickset(o.AMFO - spl.without);
-   print "\n   strictlyInside=", ffmtnickset(set x <- o.AMFO | strictlyInside(x, m.o));
-   print "\n           inside=", ffmtnickset(set x <- o.AMFO | strictlyInside(x, m.o));
-nl();
-
-   if ((set x <- o.AMFO | inside(x, m.o)) == {})
-      { print " (only outside, carrying on anyway to see what the FUCK happens)\n"; }
-//    { print " (only outside, skipping)\n"; return; }
-    else { nl(); }
-
-    print "   processing..\n";
-    print "   within " + fmtamfosso(o), "\n";
-    nl();
-
-
-
-
-    var reconnected := mapfo(o.AMFO, m);
-
-    if (reconnected != obj2sso(m.m[o]) )
-    {
-      print "FUCK fuck FUCK fuck FUCK fuck FUCK fuck FUCK fuck FUCK fuck FUCK fuck \n";
-      print "FUCK fuck FUCK fuck FUCK fuck FUCK fuck FUCK fuck FUCK fuck FUCK fuck \n";
-    }
-
-    print "   done " + o.nick, " translated  SSO=", ffmtsso(reconnected),             "\n";
-    print "        " + o.nick, " direct      SSO=", ffmtsso(obj2sso(m.m[o])),         "\n";
-    print "        " + o.nick, " mapfo_INNER SSO=", ffmtsso(mapfo_INNER(o.AMFO, m)),  "\n";
-    print "        " + o.nick, " mapfo_INNER+SSO=", ffmtsso(mapfo_INNER(o.AMFO, m) +  obj2sso(m.m[m.o])),  "\n";
-    print "        " + o.nick, " mapfo_orig  SSO=", ffmtsso(mapfo_orig(o.AMFO, m)),   "\n";
-
-    nl();
-
-    print "SPORRAN: ",  o.nick + " " + sporrel(o,m) + "                            rivet.AMFX=", ffmtnickset(o.AMFX); nl();
-    print "SPORRAN: ",  o.nick + " " + sporrel(o,m) + "                       sporamfx(rivet)=", ffmtnickset(sporamfx(o)); nl();
-    print "SPORRAN: ",  o.nick + " " + sporrel(o,m) + "                           trivet.AMFX=", ffmtnickset(m.m[o].AMFX); nl();
-    print "SPORRAN: ",  o.nick + " " + sporrel(o,m) + "                      sporamfx(trivet)=", ffmtnickset(sporamfx(m.m[o])); nl();
-    print "SPORRAN: ",  o.nick + " " + sporrel(o,m) + "             ownr2sso(sporamfx(trivet)=", ffmtsso(ownr2sso(sporamfx(m.m[o]))); nl();
-    print "SPORRAN: ",  o.nick + " " + sporrel(o,m) + "  ownr2sso(sporamfx(objThruKlon(o,m)))=", ffmtsso(ownr2sso(sporamfx(objThruKlon(o,m)))); nl();
-    print "SPORRAN: ",  o.nick + " " + sporrel(o,m) + "  ownr2sso(mapThruKlon(sporamfx(o),m))=", ffmtsso(ownr2sso(mapThruKlon(sporamfx(o),m))); nl();
-    print "SPORRAN: ",  o.nick + " " + sporrel(o,m) + "    ownr2sso(mapfoSide(sporamfx(o),m))=", ffmtsso(ownr2sso(mapfoSide(sporamfx(o),m))); nl();
-    print "SPORRAN: ",  o.nick + " " + sporrel(o,m) + "                  mapfo(sporamfx(o),m)=", ffmtsso(mapfo(sporamfx(o),m)); nl();
-
- }
-
-
-lemma {:verify false}  GEownr(
-   p : SSO, w : SSO, mp : SSO , mw : SSO, m : Klon)
-   requires HighCalidFragilistic(m)
-       requires forall o <- concensso(p)  :: m.objectReadyInKlown(o)
-       requires forall o <- concensso(w)  :: m.objectReadyInKlown(o)
-       requires forall o <- concensso(mp) :: m.objectReadyInKlown(o)
-       requires forall o <- concensso(mw) :: m.objectReadyInKlown(o)
-       requires p >= w
-
-       requires mp == mapfo(concensso(p), m)
-       requires mw == mapfo(concensso(w), m)
-
-       ensures mp >= mw
-   {
-
-   }
-
-
-
-function parameterstk(os : Owner, m : Klon) : Owner
-  requires os <= m.m.Keys
-  reads m.oHeap, m.m.Values
-{ set o <- os :: m.m[o] }
-
-function mtk(os : Owner, m : Klon) : Owner
-  requires os <= m.m.Keys
-  reads m.oHeap, m.m.Values
-{ set o <- os :: m.m[o] }
-
-function mZk(os : Owner, m : Klon) : Owner
-  requires m.SuperCalidFragilistic()
-  requires os <= m.m.Keys
-  reads m.oHeap, m.m.Values
-  { if (os >= m.o.AMFO)
-     then (MINNER(os, m))
-     else (os) }
-
-function {:isolate_assertions}  msp(ko : OWNR, m : Klon) : OWNR
-  //map sporrelOWNR
-  requires ko <= m.m.Keys
-  requires m.SuperCalidFragilistic()
-  requires m.apoCalidse()
-  requires AllReady(ko)
-  requires isFlat(ko)
-     reads m.oHeap, m.m.Values
- {
-   if (ko == m.o.AMFO) then (m.m[m.o].AMFO)
-     else if (not(ko >= m.o.AMFO))
-       then (ko)
-       else (MINNER(ko, m))
- }
-
-
-
-function {:isolate_assertions}  pOb(k : Object, m : Klon) : OWNR
-  requires {k} <= m.m.Keys
-  requires m.SuperCalidFragilistic()
-  requires m.apoCalidse()
-  requires AllReady({k})
-     reads m.oHeap, m.m.Values
- {
-  if (k == m.o) then (m.m[m.o].AMFO) else
-      (  if (outside(k,m.o))
-        then (sporamfo(k))
-        else (set z <- MINNER({k},m), zz9 <- sporamfo(z) :: zz9)  )
- }
-
-
-
-function {:isolate_assertions}  pOW(ko : OWNR, m : Klon) : OWNR
-  ///this is too much of a hack
-   requires ko <= m.m.Keys
-  requires m.SuperCalidFragilistic()
-  requires m.apoCalidse()
-  requires AllReady(ko)
-  requires isFlat(ko)
-     reads m.oHeap, m.m.Values
- {
-   if (ko == m.o.AMFO) then (m.m[m.o].AMFO)
-     else
-   if (ko == m.o.AMFB) then (m.m[m.o].AMFB)
-    else
-   if (ko == m.o.AMFX) then (m.m[m.o].AMFX)
-     else if (not(ko >= m.o.AMFO))
-       then (ko)
-       else (MINNER(ko, m))
- }
-
-
-function MINNER(os : Owner, m : Klon) : Owner
-  requires m.SuperCalidFragilistic()
-  //compare mapfo_SIDEWAYS / _INNER
-  requires os <= m.m.Keys
-  reads m.oHeap, m.m.Values
-  {(set o <- (os - m.o.AMFO) :: m.m[o]) + m.m[m.o].AMFO }
-
-  /////////////////////////////////////////////////////////////////////////////////////////////////////////////
-
-
-function {:isolate_assertions}  zzX(k : Object, m : Klon) : OWNR
-  requires {k} <= m.m.Keys
-  requires m.SuperCalidFragilistic()
-  requires m.apoCalidse()
-  requires AllReady({k})
-     reads m.oHeap, m.m.Values
- {
-  if (k == m.o) then (m.m[m.o].AMFO) else
-      (  if (outside(k,m.o))
-        then (sporamfo(k))
-        else (set z <- MINNER({k},m), zz9 <- sporamfo(z) :: zz9)  )
- }
-
-
-
-
-
-
-  ///////////////////////////////////////////////////////////////////////////////////////////////////////////
-
-function pvtself(o : Object, m : Klon) : Owner {if (o == m.o) then (m.clowner+{m.m[o]}) else (mtk(o.self,m))}
-function pvtowner(o : Object, m : Klon) : Owner {if (o == m.o) then (m.clowner)          else (mtk(o.owner,m))}
-function pvtbound(o : Object, m : Klon) : Owner {if (o == m.o) then (m.clbound)          else (mtk(o.bound,m))}
-
-function xvtself(o : Object, m : Klon) : Owner {if (o == m.o) then ({})          else (mtk(o.self,m))}
-function xvtowner(o : Object, m : Klon) : Owner {if (o == m.o) then ({})          else (mtk(o.owner,m))}
-function xvtbound(o : Object, m : Klon) : Owner {if (o == m.o) then ({})          else (mtk(o.bound,m))}
-
-  ///////////////////////////////////////////////////////////////////////////////////////////////////////////
-
- method   {:verify false}  do_object_mod4(k : Object, m : Klon)
-   requires m.objectReadyInKlown(k)
-   requires HighCalidFragilistic(m)
-   requires m.SuperCalidFragilistic()
-    ensures m.Calid()   //no fucking idea wwhy this is failing,  but qutie curious!
-    ensures m.AllLinesCalid()
- {
-   var v := m.m[k];
-   print "^^^^^^^^^^^^^^^^^^^^^^^^^^^^^^^^^^^^^^^^^^^^^^^^^^^^^^^^^^^^^^^^^^^^^^^^^^^\n";
-   print "object ", sporrel(k,m), " ", k.nick, " ~> ", v.nick, "    ",ffmtnickset(k.AMFO),"~",ffmtnickset(v.AMFO),"      ", (v.AMFO  >= v.AMFB  >= k.AMFB);   nl();
-
-if (k == m.o) { print "PIBOTTTOTION  PIVOT\n"; } else { return; }
-
-print "clowner=", ffmtnickset(m.clowner), "  clbound=", ffmtnickset(m.clbound); nl();
-
-//    print "   k.owner=", ffmtnickset(k.owner);
-//    print " k.bound=", ffmtnickset(k.bound);nl();
-//    print " k.AMFO=", ffmtnickset(k.AMFO);
-//    print " k.AMFX=", ffmtnickset(k.AMFX);
-//    print " k.AMFB=", ffmtnickset(k.AMFB);
-//    print "  ", sporamfo(k)==k.AMFO," ", (sporamfx(k)==k.AMFX)," ", sporamfb(k)==k.AMFB;
-//    nl();
-//
-//
-//    print "   v.owner=", ffmtnickset(v.owner);
-//    print " v.bound=", ffmtnickset(v.bound);nl();
-//    print " v.AMFO=", ffmtnickset(v.AMFO);
-//    print " v.AMFX=", ffmtnickset(v.AMFX);
-//    print " v.AMFB=", ffmtnickset(v.AMFB);
-//    print "  ", sporamfo(v)==v.AMFO," ", (sporamfx(v)==v.AMFX)," ", sporamfb(v)==v.AMFB;
-//    nl();
-//
-
-  //  print " ", mtk(k.self, m) == v.self, " ", mtk(k.owner, m) == v.owner, " ", mtk(k.bound, m) == v.bound;
-  //  print " ", mZk(k.AMFO, m) == v.AMFO, " ", mZk(k.AMFX, m)  == v.AMFX, " ", mZk(k.AMFB, m) == v.AMFB;
-  //  nl();
-  //  nl();
-  //  print " ", msp(k.AMFO, m) == v.AMFO, " ", msp(k.AMFX, m)  == v.AMFX, " ", msp(k.AMFB, m) == v.AMFB;
-//   nl();
-
-   print "k  : ", ffmtnickset(k.self), " ", ffmtnickset(k.owner), " ", ffmtnickset(k.bound); nl();
-
-
-   print "v  : ", ffmtnickset(v.self), " ", ffmtnickset(v.owner), " ", ffmtnickset(v.bound); nl();
-   print "pvt: ", ffmtnickset(pvtself(k,m)), " ", ffmtnickset(pvtowner(k,m)), " ", ffmtnickset(pvtbound(k,m)); nl();
-
-   print "xvt: ", ffmtnickset(xvtself(k,m)), " ", ffmtnickset(xvtowner(k,m)), " ", ffmtnickset(xvtbound(k,m)); nl();
-
-
-
-   print "KLON ", ffmtnickset(m.clowner+{v}), " ", ffmtnickset(m.clowner), " ", ffmtnickset(m.clbound); nl();
-
-
-   print "pvt: ", pvtself(k,m) == v.self, " ", pvtowner(k,m) == v.owner, " ", pvtbound(k,m) == v.bound;
-   print "|", sporamfo(m.m[k]) == v.AMFO, " ", sporamfx(m.m[k])  == v.AMFX, " ", sporamfb(m.m[k]) == v.AMFB; nl();
-  //  print "mtk: ", mtk(k.self, m) == v.self, " ", mtk(k.owner, m) == v.owner, " ", mtk(k.bound, m) == v.bound;
-//    print "|", mtk(k.AMFO, m) == v.AMFO, " ", mtk(k.AMFX, m)  == v.AMFX, " ", mtk(k.AMFB, m) == v.AMFB; nl();
-//
-//
-//    print "mZk: ", mZk(k.self, m) == v.self, " ", mZk(k.owner, m) == v.owner, " ", mZk(k.bound, m) == v.bound;
-//    print "|", mZk(k.AMFO, m) == v.AMFO, " ", mZk(k.AMFX, m)  == v.AMFX, " ", mZk(k.AMFB, m) == v.AMFB; nl();
-//
-//    print "msp: ", msp(k.self, m) == v.self, " ", msp(k.owner, m) == v.owner, " ", msp(k.bound, m) == v.bound;
-//    print "|", msp(k.AMFO, m) == v.AMFO, " ", msp(k.AMFX, m)  == v.AMFX, " ", msp(k.AMFB, m) == v.AMFB; nl();
-// //
-//    print "pOb: ", pOb(k, m) == v.self, " ", pOb(k, m) == v.owner, " ", pOb(k, m) == v.bound;
-//    print "|", pOb(k, m) == v.AMFO, " ", pOb(k, m)  == v.AMFX, " ", pOb(k, m) == v.AMFB; nl();
-//
-//    print "pOW: ", pOW(k.self, m) == v.self, " ", pOW(k.owner, m) == v.owner, " ", pOW(k.bound, m) == v.bound;
-//    print "|", pOW(k.AMFO, m) == v.AMFO, " ", pOW(k.AMFX, m)  == v.AMFX, " ", pOW(k.AMFB, m) == v.AMFB; nl();
-
-   print "zzz: ", mtk(k.self, m) == v.self, " ", mtk(k.owner, m) == v.owner, " ", mtk(k.bound, m) == v.bound;
-   print "|", sporamfo(m.m[k]) == v.AMFO, " ", sporamfx(m.m[k])  == v.AMFX, " ", sporamfb(m.m[k]) == v.AMFB; nl();
-
-   print "zzz: ",ffmtnickset(mtk(k.self, m)), " ",ffmtnickset(mtk(k.owner, m)), " ",ffmtnickset(mtk(k.bound, m));
-   print "|",ffmtnickset(sporamfo(m.m[k])), " ",ffmtnickset(sporamfx(m.m[k])), " ",ffmtnickset(sporamfb(m.m[k])); nl();
-//
-//
-//    print "zz9: ", mtk(k.self, m) == v.self, " ", mtk(k.owner, m) == v.owner, " ", mtk(k.bound, m) == v.bound;
-//    print "|", splatten(mtk(k.owner,m)+{m.m[k]}) == v.AMFO, " ", splatten(mtk(k.owner,m)) == v.AMFX, " ", splatten(mtk(k.bound,m)) == v.AMFB; nl();
-//
-
-
-   print "zz8: ", mtk(k.self, m) == v.self, " ", mtk(k.owner, m) == v.owner, " ", mtk(k.bound, m) == v.bound;
-   print "|", splatten(m.m[k].owner)+{m.m[k]} == v.AMFO, " ", splatten(m.m[k].owner) == v.AMFX, " ", splatten(m.m[k].bound) == v.AMFB; nl();
-
-//    print "mfo:", mapfo(k.self, m) == ownr2sso(v.self), " ", mapfo(k.owner, m) == ownr2sso(v.owner), " ", mapfo(k.bound, m) == ownr2sso(v.bound);
-//    print "|", (mapfo(k.AMFO,m)) == ownr2sso(v.AMFO), " ", (mapfo(k.AMFX,m)) == ownr2sso(v.AMFX), " ", (mapfo(k.AMFB,m)) == ownr2sso(v.AMFB); nl();
-// //
-//4
-//    print "msp: ", mtk(k.self, m) == v.self, " ", mtk(k.owner, m) == v.owner, " ", mtk(k.bound, m) == v.bound;
-//    print "|", splatten(mtk(k.owner,m)+{m.m[k]}) == v.AMFO, " ", splatten(mtk(k.owner,m)) == v.AMFX, " ", splatten(mtk(k.bound,m)) == v.AMFB; nl();
-
-
-
-  //  ensures sporamfo(o) == splatten(o.owner)+{o}
-  //  ensures sporamfx(o) == splatten(o.owner)
-  //  ensures sporamfb(o) == splatten(o.bound)
-
-    var reconnected := mapfo(k.AMFO, m);
-
-    if (reconnected != obj2sso(m.m[k]) )
-    {
-      print "FUCK fuck FUCK fuck FUCK fuck FUCK fuck FUCK fuck FUCK fuck FUCK fuck \n";
-      print "FUCK fuck FUCK fuck FUCK fuck FUCK fuck FUCK fuck FUCK fuck FUCK fuck \n";
-    }
-
-
-
-
-   print "vvvvvvvvvvvvvvvvvvvvvvvvvvvvvvvvvvvvvvvvvvvvvvvvvvvvvvvvvvvvvvvvvvvvvvvvvvv\n\n";
-
- }
-
-
-//{:timeLimit 60}
-lemma {:isolate_assertions} MapfoPLUS1(oo1 : OWNR, oo2 : OWNR, o : Object, m : Klon)
-   requires HighCalidFragilistic(m)
-   requires forall o <- oo1     :: m.objectReadyInKlown(o)
-   requires forall o <- oo2     :: m.objectReadyInKlown(o)
-    ensures mapfo(oo1 + oo2,m ) == mapfo(oo1,m) + mapfo(oo2,m)
-
-    requires oo2 == {o}
-   {
-     if (o in oo1) {
-      setfuck(oo1, oo2, o);
-      assert (oo1 + oo2) == (oo1 + {o}) == oo1;
-      assert mapfo(oo1 + oo2,m ) == mapfo(oo1,m) + mapfo(oo2,m);
-      return;
-     }
-     assert o !in oo1;
-   }
-
-
-lemma {:isolate_assertions} MapfoNULL(m : Klon)
-   requires HighCalidFragilistic(m)
-    ensures mapfo({}, m) == {}
-{}
-
-lemma {:isolate_assertions} SSOofNULL()
-    ensures ownr2sso({}) == {}
-{}
-
-lemma {:isolate_assertions} SSO_GT(oo1 : OWNR, oo2 : OWNR, m : Klon)
-   requires HighCalidFragilistic(m)
-   requires forall o <- oo1     :: m.objectReadyInKlown(o)
-   requires forall o <- oo2     :: m.objectReadyInKlown(o)
-   requires isFlat(oo1)
-   requires isFlat(oo2)
-   requires oo2 <= oo1
-    ensures ownr2sso(oo2) <= ownr2sso(oo1)
-   {}
-
-
-
-
-
-
-lemma {:isolate_assertions} MapfoPLUS2(oo1 : OWNR, oo2 : OWNR, o : Object, m : Klon)
-   requires HighCalidFragilistic(m)
-   requires forall o <- oo1     :: m.objectReadyInKlown(o)
-   requires forall o <- oo2     :: m.objectReadyInKlown(o)
-   requires isFlat(oo1)
-   requires isFlat(oo2)
-    requires oo2 == {o}
-    requires o in oo1
-     ensures oo2 <= oo1
-//     ensures mapfo(oo2,m) <= mapfo(oo1,m)
-   {
-
-assert oo2 <= oo1;
-assert ownr2sso(oo2) <= ownr2sso(oo1);
-// assert  (set o <- oo2 | inside(o, m.o)) <= (set o <- oo1 | inside(o, m.o));
-// assert ((set o <- oo1 | inside(o, m.o)) == {}) ==> ((set o <- oo2 | inside(o, m.o)) == {});
-
-assert (set o <- oo2 |  inside(o, m.o)) <= (set o <- oo1 |  inside(o, m.o));
-assert (set o <- oo2 | outside(o, m.o)) <= (set o <- oo1 | outside(o, m.o));
-
-
-if ((set o <- oo1 | inside(o, m.o)) == {})
-   {
-    assert mapfo(oo1,m) == ownr2sso(oo1);
-    assert oo2 <= oo1;
-    assert (set o <- oo2 | inside(o, m.o)) == {};
-    assert mapfo(oo2,m) == ownr2sso(oo2);
-    assert ownr2sso(oo2) <= ownr2sso(oo1);
-    assert mapfo(oo2,m) <= mapfo(oo1,m);
-    return;
-   }
-
-assert (set o <- oo1 | inside(o, m.o)) != {};
-
-// if ((set o <- oo2 | inside(o, m.o)) == {})
-//  {
-//
-//   assert mapfo(oo2,m) <= mapfo(oo1,m);
-//   return;
-//  }
-
-assert ((set o <- oo1 | inside(o, m.o)) != {}) && ((set o <- oo2 | inside(o, m.o)) != {});
-
-assert (set o <- oo2 |  inside(o, m.o)) <= (set o <- oo1 |  inside(o, m.o));
-assert (set o <- oo2 | outside(o, m.o)) <= (set o <- oo1 | outside(o, m.o));
-
-
-
-assert (oo2 - m.o.AMFO) <= (oo1 - m.o.AMFO);
-assert forall y <- (oo2 - m.o.AMFO) :: y in (oo1 - m.o.AMFO);
-
-assert mapfo_INNER(oo2,m) <= mapfo_INNER(oo1,m);
-
-assert (mapfo_INNER(oo2,m) + obj2sso(m.m[m.o])) <= (mapfo_INNER(oo1,m) + obj2sso(m.m[m.o]));
-
-assert mapfo(oo1,m) == (mapfo_INNER(oo1,m) + obj2sso(m.m[m.o]));
-assert mapfo(oo2,m) == (mapfo_INNER(oo2,m) + obj2sso(m.m[m.o]));
-
-//
-// assert
-//   (if ((set o <- oo2 | inside(o, m.o)) == {}) then ownr2sso(oo2) else (mapfo_INNER(oo2,m)) + obj2sso(m.m[m.o]))
-//   <=
-//   (if ((set o <- oo1 | inside(o, m.o)) == {}) then ownr2sso(oo1) else (mapfo_INNER(oo1,m)) + obj2sso(m.m[m.o]))
-//   ;
-
-
-
-assert mapfo(oo2,m) <= mapfo(oo1,m);
-
-   }
-
-lemma setfuck(oo1 : OWNR, oo2 : OWNR, o : Object)
-    requires oo2 == {o}
-    requires o in oo1
-     ensures oo1 + {o} == oo1
-     ensures oo1 + oo2 == oo1
-{}
-
-lemma setcrap(oo1 : OWNR, oo2 : OWNR, x : OWNR)
-    requires oo2 <= oo1
-     ensures (oo2+x) <= (oo1+x)
-{}
-
-
-lemma {:isolate_assertions} {:resource_limit 32000000} INSIDEOUT(oo : OWNR, m : Klon)
-   requires forall o <- oo :: m.objectReadyInKlown(o)
-   requires oo <= m.m.Keys
-   requires HighCalidFragilistic(m)
-    ensures ((set o <- oo | inside(o, m.o)) == {})  ==> (forall o <- oo :: outside(o, m.o))
-    ensures ((set o <- oo | inside(o, m.o)) == {}) <==  (forall o <- oo :: outside(o, m.o))
-
-    ensures ((set o <- oo | inside(o, m.o)) >  {})  ==> (exists o <- oo :: inside(o, m.o))
-    ensures ((set o <- oo | inside(o, m.o)) >  {}) <==  (exists o <- oo :: inside(o, m.o))
-
-    ensures ((set o <- oo | inside(o, m.o)) >  {})  ==> (not (forall o <- oo :: outside(o, m.o)))
-    ensures ((set o <- oo | inside(o, m.o)) >  {}) <==  (not (forall o <- oo :: outside(o, m.o)))
- {}
-
-lemma {:isolate_assertions} MapfoEQ(oo1 : OWNR, oo2 : OWNR, m : Klon)
-   requires HighCalidFragilistic(m)
-   requires forall o <- oo1  :: m.objectReadyInKlown(o)
-   requires forall o <- oo2  :: m.objectReadyInKlown(o)
-    ensures (oo1 == oo2)  ==> (mapfo(oo1,m) == mapfo(oo2,m))
- //   ensures (oo1 == oo2) <==  (mapfo(oo1,m) == mapfo(oo2,m))
-   {}
-
-
-lemma {:isolate_assertions} MapfoEQ2(o1 : Object, o2 : Object, m : Klon)
-   requires HighCalidFragilistic(m)
-   requires m.objectReadyInKlown(o1)
-   requires m.objectReadyInKlown(o2)
-    ensures (o1 == o2)  ==> (mapfo(o1.AMFO,m) == mapfo(o2.AMFO,m))
-  //  ensures (o1 == o2) <==  (mapfo(o1.AMFO,m) == mapfo(o2.AMFO,m))
-   {}
-
-
- function {:isolate_assertions} {:timeLimit 20} mapfo_orig(oo : OWNR, m : Klon) : SSO
-   requires forall o <- oo :: m.objectReadyInKlown(o)
-   requires oo <= m.m.Keys
-   requires HighCalidFragilistic(m)
-    ensures                 m.o.AMFO <= m.m.Keys
-    ensures forall o <- oo :: o.AMFO <= m.m.Keys
-   reads oo, m.m.Keys, m.m.Values, m.oHeap
- {
-   if ((set o : Object <- oo | inside(o, m.o)) == {}) then ownr2sso(oo) else
-
-    (( set y : Object <- (oo - m.o.AMFO) ::
-
-       if (y.AMFO >= m.o.AMFO) then
-         (mapThruKlon( (y.AMFO - m.o.AMFO), m ) +  ( m.m[m.o].AMFO )
-         ) else ( y.AMFO
-          )
-      ) + obj2sso(m.m[m.o]))
-
- }
-
-
-
-
-
-lemma {:isolate_assertions} MAPFO_MAPFO_ORIG1(oo : OWNR, m : Klon)
-   requires forall o <- oo :: m.objectReadyInKlown(o)
-   requires oo <= m.m.Keys
-   requires HighCalidFragilistic(m)
-    ensures mapfo(oo,m) == mapfo_orig(oo,m)
-   { }
-
-
-lemma {:isolate_assertions}  {:timeLimit 120} MAPFO_MAPFO_ORIG2(oo : OWNR, m : Klon)
-   requires forall o <- oo :: m.objectReadyInKlown(o)
-   requires oo <= m.m.Keys
-   requires HighCalidFragilistic(m)
-    ensures mapfo_INNER(oo,m) == mapfo_INNER_NEW(oo,m)
-   { }
-
-lemma {:isolate_assertions}  MAPFO_MAPFO_INNER1(oo : OWNR, m : Klon)
- //if there is at least one inside
- //then we're calling INNER & added into m.m[m.o]
-   requires forall o <- oo :: m.objectReadyInKlown(o)
-   requires oo <= m.m.Keys
-   requires HighCalidFragilistic(m)
-   requires ((set o <- oo | inside(o, m.o)) > {})
-    ensures mapfo(oo,m) == (mapfo_INNER(oo,m) + obj2sso(m.m[m.o]))
-   { }
-
-//{:resource_limit 32000000}
-lemma {:isolate_assertions} MAPFO_MAPFO_INNER2(oo : OWNR, m : Klon)
-//if all items are outside m.o they go straight through
-   requires forall o <- oo :: m.objectReadyInKlown(o)
-   requires oo <= m.m.Keys
-   requires HighCalidFragilistic(m)
-
-   requires forall o <- oo :: outside(o, m.o)
-   requires oo !! m.o.AMFO
-    ensures mapfo(oo,m)       == ownr2sso(oo)
-//    ensures mapfo_INNER(oo,m) >= ownr2sso(oo)  //NOT this... *********
-  {}
-
-//
-// lemma {:isolate_assertions} MAPFO_MAPFO_INNER3(oo : OWNR, m : Klon)
-// //all items outside m.o go straight through!
-//    requires forall o <- oo :: m.objectReadyInKlown(o)
-//    requires oo <= m.m.Keys
-//    requires HighCalidFragilistic(m)
-//
-//     ensures forall o <- oo | strictlyInside(o, m.o) ::
-//        (mapfo_SIDEWAYS(o,m) in mapfo(oo,m))
-//   {
-//
-//   }
-
-
-
-lemma {:isolate_assertions}  MAPFO_MAPFO_INNER8(oo : OWNR, m : Klon, r : SSO, i : SSO)
-//incomplete.  does nothing.
-//OK now does the same as GT3i???
-   requires forall o <- oo :: m.objectReadyInKlown(o)
-   requires oo <= m.m.Keys
-   requires HighCalidFragilistic(m)
-   requires r == mapfo(oo,m)
-   requires i == mapfo_INNER(oo,m)
-
-   requires ((set o <- oo | inside(o, m.o)) > {})   //at least something is inside, so we go down that way. b
-
-   ensures mapfo(oo,m) == (mapfo_INNER(oo,m) + obj2sso(m.m[m.o]))
-   { }
-
-// lemma {:isolate_assertions} {:timeLimit 20} MAPFO_MAPFO_INNER9(oo : OWNR, m : Klon)
-//  //DOESNT, SHOULDNT, CANT WORK. THIS IS A BIT STUPID INNIT??
-//    requires forall o <- oo :: m.objectReadyInKlown(o)
-//    requires oo <= m.m.Keys
-//    requires HighCalidFragilistic(m)
-//
-//    requires ((set o <- oo | outside(o, m.o)) > {})
-//    // ensures mapfo(oo,m) == (mapfo_INNER(oo,m) + obj2sso(m.m[m.o]))
-//    {
-//     assert forall o <- oo :: outside(o, m.o);
-//     assert forall o <- oo :: not(o.AMFO >= m.o.AMFO);
-//     assert not( outside(m.o, m.o) );
-//     assert not(m.o.AMFO <= oo);
-//
-//    }
-
-
-
-
-//{:resource_limit 32000000}
-lemma {:isolate_assertions} MAPFO_MAPFO_GT1(oo1 : OWNR, oo2 : OWNR, m : Klon)
-  //mapfo_SIDEWAYS maintains <= (modulo preconditions)
-   requires forall o <- oo1 :: m.objectReadyInKlown(o)
-   requires forall o <- oo2 :: m.objectReadyInKlown(o)
-   requires oo1 <= m.m.Keys
-   requires oo2 <= m.m.Keys
-   requires isFlat(oo1)
-   requires isFlat(oo2)
-   requires HighCalidFragilistic(m)
-   requires oo2 <= oo1
-   requires forall o <- oo1 :: (o !in m.o.AMFO) && (inside(o, m.o))
-    ensures forall o <- oo2 :: (o !in m.o.AMFO) && (inside(o, m.o))
-    ensures (set o <- oo2 :: mapfo_SIDEWAYS(o,m)) <=
-                     (set o <- oo1 :: mapfo_SIDEWAYS(o,m))
-  { }
-
-
-//{:resource_limit 32000000}
-lemma {:isolate_assertions} MAPFO_MAPFO_GT2(oo1 : OWNR, oo2 : OWNR, m : Klon)
- //mapfo Inner maintains <=
-   requires forall o <- oo1 :: m.objectReadyInKlown(o)
-   requires forall o <- oo2 :: m.objectReadyInKlown(o)
-   requires oo1 <= m.m.Keys
-   requires oo2 <= m.m.Keys
-   requires isFlat(oo1)
-   requires isFlat(oo2)
-   requires HighCalidFragilistic(m)
-   requires oo2 <= oo1
-
-    ensures mapfo_INNER(oo2,m) <= mapfo_INNER(oo1,m)
-    ensures (mapfo_INNER(oo2,m) + obj2sso(m.m[m.o])) <= (mapfo_INNER(oo1,m) + obj2sso(m.m[m.o]))
-{}
-
-
-lemma {:isolate_assertions} MAPFO_MAPFO_GT2thru(oo : OWNR, ext : Object, m : Klon)
-   requires forall o <- oo :: m.objectReadyInKlown(o)
-   requires oo <= m.m.Keys
-   requires isFlat(oo)
-   requires HighCalidFragilistic(m)
-   requires not(ext in m.o.AMFO) //?????
-   requires not(ext.AMFO >= m.o.AMFO)
-   requires ext in oo
-    ensures ext.AMFO in mapfo_INNER(oo,m)
-{}
-
-
-
-lemma {:isolate_assertions} MAPFO_MAPFO_GT2thru2(oo1 : OWNR, oo2 : OWNR, ext : Object, m : Klon)
-   requires forall o <- oo1 :: m.objectReadyInKlown(o)
-   requires forall o <- oo2 :: m.objectReadyInKlown(o)
-   requires oo1 <= m.m.Keys
-   requires oo2 <= m.m.Keys
-   requires isFlat(oo1)
-   requires isFlat(oo2)
-   requires HighCalidFragilistic(m)
-   requires oo2 <= oo1
-
-   requires not(ext in m.o.AMFO) //?????
-   requires not(ext.AMFO >= m.o.AMFO)
-   requires ext in oo2
-    ensures ext in oo1
-    ensures ext.AMFO in mapfo_INNER(oo2,m)
-    ensures ext.AMFO in mapfo_INNER(oo1,m)
-{}
-
-
-
-lemma {:isolate_assertions} MAPFO_MAPFO_GT2thrall(oo1 : OWNR, oo2 : OWNR, ext : Object, m : Klon)
-   requires forall o <- oo1 :: m.objectReadyInKlown(o)
-   requires forall o <- oo2 :: m.objectReadyInKlown(o)
-   requires oo1 <= m.m.Keys
-   requires oo2 <= m.m.Keys
-   requires isFlat(oo1)
-   requires isFlat(oo2)
-   requires HighCalidFragilistic(m)
-   requires oo2 <= oo1
-
-   requires not(ext in m.o.AMFO) //?????
-   requires not(ext.AMFO >= m.o.AMFO)
-   requires ext in oo2
-    ensures ext in oo1
-    ensures ext.AMFO in mapfo_INNER(oo2,m)
-    ensures ext.AMFO in mapfo_INNER(oo1,m)
-{}
-
-
-
-
-lemma {:isolate_assertions} MAPFO_MAPFO_GT3(oo1 : OWNR, oo2 : OWNR, m : Klon)
-  //supposed to be mapfo maintains <=? in all cases?
-   requires forall o <- oo1 :: m.objectReadyInKlown(o)
-   requires forall o <- oo2 :: m.objectReadyInKlown(o)
-   requires oo1 <= m.m.Keys
-   requires oo2 <= m.m.Keys
-   requires isFlat(oo1)
-   requires isFlat(oo2)
-   requires HighCalidFragilistic(m)
-   requires oo2 <= oo1
-
-  //  ensures mapfo(oo2,m) <= mapfo(oo1,m)
-{
-  //if oo1 is all outside pivot, so must be oo2 - and yourdon.
-  if ((set o <- oo1 | inside(o, m.o)) == {})  //forall o <- oo1 :: outside(o, m.o)
-     {
-      assert ((set o <- oo2 | inside(o, m.o)) == {}); // //forall o <- oo1 :: outside(o, m.o)
-
-      assert ownr2sso(oo2) <= ownr2sso(oo1);
-      assert mapfo(oo2,m) <= mapfo(oo1,m);
-      return;
-     }
-
-    //oo1 does have something inside.
-    assert ((set o <- oo1 | inside(o, m.o)) > {});
-
-
-  //if set2 *also* has something inside then we're both going thru inner
-  if ((set o <- oo2 | inside(o, m.o)) > {})
-     {
-      assert ((set o <- oo2 | inside(o, m.o)) > {});
-      assert OO2IN: ((set o <- oo2 | inside(o, m.o)) > {});
-      assert ((set o <- oo1 | inside(o, m.o)) > {});
-      assert oo2 <= oo1;
-      MAPFO_MAPFO_GT2(oo1,oo2,m);
-      assert
-        (mapfo_INNER(oo2,m) + obj2sso(m.m[m.o]))
-           <= (mapfo_INNER(oo1,m) + obj2sso(m.m[m.o]));
-
-      MAPFO_MAPFO_GT3i(oo1,m);
-      assert ((set o <- oo2 | inside(o, m.o)) > {}) by { reveal OO2IN; }
-      MAPFO_MAPFO_GT3i(oo2,m);
-      assert mapfo(oo1,m) == (mapfo_INNER(oo1,m) + obj2sso(m.m[m.o]));
-      assert mapfo(oo2,m) == (mapfo_INNER(oo2,m) + obj2sso(m.m[m.o]));
-      MAPFO_MAPFO_GT2(oo1,oo2,m);
-      assert mapfo(oo2,m) <= mapfo(oo1,m);
-      return;
-     }
-
-  //at this poiint oo1 definitely HAS something inside and goes down thru INNER
-  //but oo2 DOES NOT.
-  assert oo2 <= oo1;
-  assert ((set o <- oo1 | inside(o, m.o)) >  {});
-  assert ((set o <- oo2 | inside(o, m.o)) == {});
-//  assert ((set o <- oo2 | outside(o,m.o)) == oo2);
-// assert forall o <- oo2 :: outside(o, m.o);
-
-
-MAPFO_MAPFO_GT3x(oo1,oo2,m);
-assert mapfo(oo2,m) <= mapfo(oo1,m);
-}
-
-
-lemma {:isolate_assertions} MAPFO_MAPFO_GT3i(oo : OWNR, m : Klon)
- // if there is at least one on oo inside, mapfo is Inner+thingey
-   requires forall o <- oo :: m.objectReadyInKlown(o)
-   requires oo <= m.m.Keys
-   requires isFlat(oo)
-   requires HighCalidFragilistic(m)
-   requires (set o <- oo | inside(o, m.o)) > {}   //exists o <- oo :: inside(o, m.o)
-    ensures mapfo(oo,m) == (mapfo_INNER(oo,m) + obj2sso(m.m[m.o]))
-{
-  //YAY DAFNY!!
-  // INSIDEOUT(oo,m);
-  // assert exists o <- oo :: inside(o, m.o);
-  // assert (set o <- oo | inside(o, m.o)) > {};
-  // assert mapfo(oo,m) == (mapfo_INNER(oo,m) + obj2sso(m.m[m.o]));
-
-}
-
-
-
-lemma XLEM<T(==)>(e : T, s : set<T>)
-   requires e in s
-    ensures {e} <= s
-    ensures {e} > {}
-    ensures (set o  <- s | e == o :: o) > {}
-  {}
-
-lemma YLEM<T(==)>(e : T, s : set<T>)
-   requires e in s
-    ensures {e} <= s
-    ensures {e} > {}
-    ensures (set o  <- s | {o} <= s) > {}
-  {}
-
-lemma ELEM<T(==)>(e :set<T>, s : set<set<T>>)
-   requires e in s
-    ensures {e} <= s
-    ensures {e} > {}
-    ensures (set o  <- s | {o} <= s) > {}
- {}
-
-lemma FUKSSO(oo : OWNR, sso : SSO)
-   requires oo in sso
-    ensures {oo} <= sso
-    ensures {oo} > {}
-    ensures (set o <- sso | o <= oo) > {}
- {}
-
-lemma {:isolate_assertions} {:timeLimit 15} MAPFO_MAPFO_GT3j(oo : OWNR, m : Klon)
- //one inside pivot into mapfo, at least one inside blivet out of mapfo
-   requires forall o <- oo :: m.objectReadyInKlown(o)
-   requires oo <= m.m.Keys
-   requires isFlat(oo)
-   requires HighCalidFragilistic(m)
-    ensures forall k <- m.m.Keys :: m.m[k].Ready()
-   requires (set o <- oo | inside(o, m.o)) > {}                 //exists o <- oo :: inside(o, m.o)
-    ensures (m.m[m.o].AMFO) in mapfo(oo,m)
-    ensures (set o <- mapfo(oo,m) | o  >= m.m[m.o].AMFO) > {}   //exists o <- mapfo(oo,m) :: o >= m.m[m.o].AMFO
-{
-   assert (set o <- oo | inside(o, m.o)) > {};
-   MAPFO_MAPFO_GT3i(oo,m);
-   assert mapfo(oo,m) == (mapfo_INNER(oo,m) + obj2sso(m.m[m.o]));
-  //  assert inside(m.m[m.o], m.m[m.o]);
-  //  assert m.m[m.o].Ready();
-  //  assert forall o <- m.m[m.o].AMFO :: o.Ready();
-  //  assert forall oo <- obj2sso(m.m[m.o]), o <- oo :: o.Ready();
-   assert (m.m[m.o].AMFO) in obj2sso(m.m[m.o]);
-   assert (m.m[m.o].AMFO) in mapfo(oo,m);
-   assert {m.m[m.o].AMFO} > {};
-   assert (set o <- obj2sso(m.m[m.o]) | o  >= m.m[m.o].AMFO) > {}; //FUCK
-   assert (set o <- mapfo(oo,m)       | o  >= m.m[m.o].AMFO) > {};
-}
-
-
-lemma {:isolate_assertions} MAPFO_MAPFO_GT3o(oo : OWNR, m : Klon)
- //everyting outside pivot into mapfo, nothing inside blivet outside mapfo
-   requires forall o <- oo :: m.objectReadyInKlown(o)
-   requires oo <= m.m.Keys
-   requires isFlat(oo)
-   requires HighCalidFragilistic(m)
-   requires forall o : Object <- oo :: outside(o,m.o)
-    ensures forall r : Owner <- mapfo(oo,m) :: not(r >= m.o.AMFO)
-    ensures forall r : Owner <- mapfo(oo,m) :: not(r >= m.m[m.o].AMFO)
-{}
-
-
-lemma {:isolate_assertions} {:timeLimit 30} MAPFO_MAPFO_GT3x(oo1 : OWNR, oo2 : OWNR, m : Klon)
-//IF oo2 <= oo1, AND oo1 has something inside, and oo2 does not, then mapfo oo2 <= mapfo oo1
-   requires forall o <- oo1 :: m.objectReadyInKlown(o)
-   requires forall o <- oo2 :: m.objectReadyInKlown(o)
-   requires oo1 <= m.m.Keys
-   requires oo2 <= m.m.Keys
-   requires isFlat(oo1)
-   requires isFlat(oo2)
-   requires HighCalidFragilistic(m)
-   requires oo2 <= oo1
-
-   requires (set o <- oo1 | inside(o, m.o)) >  {}    //exists o <- oo1 :: inside(o, m.o)
-   requires (set o <- oo2 | inside(o, m.o)) == {}    //requires forall o <- oo2 :: outside(o, m.o)
-   ensures mapfo(oo2,m) <= mapfo(oo1,m)
-
-{
-
-  assert oo2 <= oo1;
-  assert (set o <- oo1 | inside(o, m.o)) >  {};
-  assert (set o <- oo2 | inside(o, m.o)) == {};
-
-
-  var unicorn :| (unicorn in oo1) && (unicorn !in oo2) && (inside(unicorn, m.o));
-
-    assert unicorn.AMFO >= m.o.AMFO;
-    MAPFO_MAPFO_GT3o(oo2,m);
-    assert forall r : Owner <- mapfo(oo2,m) :: not(r >= m.o.AMFO);
-    assert forall r : Owner <- mapfo(oo2,m) :: not(r >= m.m[m.o].AMFO);
-
-    assert forall r : Owner <- mapfo(oo2,m) :: not(r >= m.m[m.o].AMFO);
-    assert unicorn.AMFO >= m.o.AMFO;
-
-assert isFlat(unicorn.AMFO);
-assert unicorn.AMFO > {};
-assert (set o <- unicorn.AMFO | o.AMFO >= m.o.AMFO) > {};
-
-MAPFO_MAPFO_GT3j(unicorn.AMFO,m);
-assert (set o <- mapfo(unicorn.AMFO,m) | o  >= m.m[m.o].AMFO) > {};
-
-assert oo2 <= oo1;
-assert (unicorn in oo1);
-assert (unicorn !in oo2);
-
-var        bicorn := mapfo({unicorn},m);
-assert     bicorn <= mapfo(oo1,m);         //WHAT THE FUCKY FUCK?
-assert not(bicorn <= mapfo(oo2,m));
-
- assert not(mapfo(oo1,m) <= mapfo(oo2,m));
-
- assert mapfo(oo2,m) <= mapfo(oo1,m);
-
-
-
-//  assert forall x : OWNR <- mapfo(oo2,m) :: not(x >= m.o.AMFO) && not(x >= m.m[m.o].AMFO);  //pivot & blivet
-
-}
+///////////////////////////////////////////////////////////////////////////////////////
 
 
 method {:isolate_assertions} {:timeLimit 30} wrangle7()
@@ -1224,7 +147,7 @@ method {:isolate_assertions} {:timeLimit 30} wrangle7()
 //pivot is b, external owner is e, orig is b,c,d, d has owner c & sideowner e, clone is k l m
   returns (t : Object, a : Object, b : Object, c : Object, d : Object, e : Object,
            k : Object, l : Object, m : Object,
-           os : set<Object>, oq : seq<Object>)
+           os : set<Object>, oq : seq<Object>, name : string)
  ensures t.Ready()
  ensures a.Ready()
  ensures b.Ready()
@@ -1238,6 +161,7 @@ method {:isolate_assertions} {:timeLimit 30} wrangle7()
 //  ensures inside(d,c)
 //  ensures inside(d,e)
  {
+    name := "wrangle7";
     print "wrangle7\n";
 
     t := new Object.make(protoTypes, {},  {},"t");
@@ -1260,7 +184,7 @@ method {:isolate_assertions} {:timeLimit 30} wrangle7()
             expect flatten(m_oo) >= flatten(m_mb);
             assert AllReady(m_oo);
             expect AllReady(m_oo);
-            assert (flatten(m_mb) >= collectBounds(flatten(m_oo)));
+//            assert (flatten(m_mb) >= collectBounds(flatten(m_oo)));
             expect (flatten(m_mb) >= collectBounds(flatten(m_oo)));
             // assume m_context >= flatten(m_oo) >= flatten(m_mb);
             // assume AllReady(m_oo);
@@ -1274,7 +198,7 @@ method {:isolate_assertions} {:timeLimit 30} wrangle7()
 
     // k := new Object.make(protoTypes, {},  {},"k");
     // l := new Object.make(protoTypes, {},  {},"l");
-    // m := new Object.make(protoTypes, {},  {},"m");
+                // m := new Object.make(protoTypes, {},  {},"m");
 
 
 
@@ -1293,43 +217,12 @@ print "m_oo= ", ffmtnickset(m_oo), "\n";
 print "flatten(m_oo)= ", ffmtnickset(flatten(m_oo)), "\n";
 print "m_mb= ", ffmtnickset(m_mb), "\n";
 print "flatten(m_mb)= ", ffmtnickset(flatten(m_mb)), "\n";
-print "collectBounds(flatten(m_oo))= ", ffmtnickset(collectBounds(flatten(m_oo))), "\n";
+//print "collectBounds(flatten(m_oo))= ", ffmtnickset(collectBounds(flatten(m_oo))), "\n";
 
 print "ctxt>=flatten(m_oo)= ", (m_context >= flatten(m_oo)), "\n";
 print "flatten(m_oo)>=flatten(m_mb)= ", (flatten(m_oo) >= flatten(m_mb)), "\n";
 print "AllReady(m_oo)= ", AllReady(m_oo), "\n";
-print "flatten(m_mb) >= collectBounds(flatten(m_oo))= ", flatten(m_mb) >= collectBounds(flatten(m_oo)), "\n";
-
-
-
-
-
-//
-//     assert forall x <- os :: x.Ready() by {
-//
-//         assert t.Ready();`
-//         assert a.Ready();
-//         assert b.Ready();
-//         assert c.Ready();
-//         assert d.Ready();
-//         assert e.Ready();
-//         assert k.Ready();
-//         assert l.Ready();
-//         assert m.Ready();
-//
-//         assert t in os;
-//         assert a in os;
-//         assert b in os;
-//         assert c in os;
-//         assert d in os;
-//         assert e in os;
-//         assert k in os;
-//         assert l in os;
-//         assert m in os;
-//
-//         assert os == {t, a, b, c, d, e, k, l, m};
-//
-//      }
+  //print "flatten(m_mb) >= collectBounds(flatten(m_oo))= ", flatten(m_mb) >= collectBounds(flatten(m_oo)), "\n";
 
 
     AllTheseFuckingObjectsAreReadyYouIdiot(t, a, b, c, d, e, k, l, m, os);
@@ -1342,6 +235,9 @@ print "flatten(m_mb) >= collectBounds(flatten(m_oo))= ", flatten(m_mb) >= collec
     print "wrdone7\n";
  }
 
+///////////////////////////////////////////////////////////////////////////////////////
+///////////////////////////////////////////////////////////////////////////////////////
+///////////////////////////////////////////////////////////////////////////////////////
 
 
 method {:isolate_assertions} jandal8()
@@ -1350,7 +246,7 @@ method {:isolate_assertions} jandal8()
 //pivot is b, external owner is e, orig is b,c,d, d has owner c & sideowner e, clone is k l m BUT now owned by **d**
   returns (t : Object, a : Object, b : Object, c : Object, d : Object, e : Object,
            k : Object, l : Object, m : Object,
-           os : set<Object>, oq : seq<Object>)
+           os : set<Object>, oq : seq<Object>, name : string)
  ensures t.Ready()
  ensures a.Ready()
  ensures b.Ready()
@@ -1365,6 +261,7 @@ method {:isolate_assertions} jandal8()
 //  ensures inside(d,e)
  {
     print "jandal8\n";
+    name := "jandal8";
 
     t := new Object.make(protoTypes, {},  {},"t");
     a := new Object.make(protoTypes, {t}, {t}, "a");
@@ -1410,7 +307,7 @@ assert flatten({d}) == {t,a,b,c,d,e};
             assert {t,a,b,c,d,e} >= flatten({d});
             assert flatten({d}) >= flatten({d});
             assert AllReady({d});
-            assert (flatten({d}) >= collectBounds(flatten({d})));
+            assert nuBoundsOK({d},{d});
     k := new Object.make(protoTypes, {d}, {t,a,b,c,d,e}, "k¢b"); //top of coone - of b
 
 /// assert k.AMFO == {t,a,b,c,d,e,k};
@@ -1421,7 +318,7 @@ assume flatten({k}) == {t,a,b,c,d,e,k};
             assert {t,a,b,c,d,e,k} >= flatten({k});
             assert flatten({k}) >= flatten({k});
             assert AllReady({k});
-            assert (flatten({k}) >= collectBounds(flatten({k})));
+            assert nuBoundsOK({k},{k});
     l := new Object.make(protoTypes, {k}, {t,a,b,c,d,e,k}, "l¢c"); //clone of c
 
 /// assert l.AMFO == {t,a,b,c,d,e,k,l};
@@ -1443,7 +340,7 @@ assume flatten({k}) == {t,a,b,c,d,e,k};
             expect flatten(m_oo) >= flatten(m_mb);
             assert AllReady(m_oo);
             expect AllReady(m_oo);
-            assert (flatten(m_mb) >= collectBounds(flatten(m_oo)));
+//            assert (flatten(m_mb) >= collectBounds(flatten(m_oo)));
             expect (flatten(m_mb) >= collectBounds(flatten(m_oo)));
             // assume m_context >= flatten(m_oo) >= flatten(m_mb);
             // assume AllReady(m_oo);
@@ -1516,36 +413,13 @@ nl();
  }
 
 
-method printAllOwnershipsAndBounds(oo : Owner, context : set<Object>, name : string, mb : Owner := oo)
-//warning - this doesn't do what it should (print stuff out of an object)
-//but prints stuff from the arguments handed in only
-{
-print "============================================================\nprintAllOwnershipsAndBounds ";
-print name, "\n";
-
-print "context= ", ffmtnickset(context), "\n";
-print "oo= ", ffmtnickset(oo), "\n";
-print "flatten(oo)= ", ffmtnickset(flatten(oo)), "\n";
-print "mb= ", ffmtnickset(mb), "\n";
-print "flatten(mb)= ", ffmtnickset(flatten(mb)), "\n";
-print "collectBounds(flatten(oo))= ", ffmtnickset(collectBounds(flatten(oo))), "\n";
-print "set oo.AMFB=", fmtsso( set oo <- flatten(mb) :: oo.AMFB  ), "\n";
-
-print "ctxt>=flatten(oo)= ", (context >= flatten(oo)), "\n";
-print "flatten(oo)>=flatten(mb)= ", (flatten(oo) >= flatten(mb)), "\n";
-print "AllReady(oo)= ", AllReady(oo), "\n";
-print "flatten(mb) >= collectBounds(flatten(oo))= ", flatten(mb) >= collectBounds(flatten(oo)), "\n";
-print "forall oo <- mb :: (flatten(mb) <= oo.AMFB)=", (forall oo <- mb :: (flatten(mb) <= oo.AMFB)) ,"\n";
-}
-
-
 method {:isolate_assertions} sandal8()
 //sets up a full-done clone *with sideways partial owners*
 //otherwise compatible with wrangle - except klone owned by d  from
 //pivot is b, external owner is e, orig is b,c,d, d has owner c & sideowner e, clone is k l m BUT now owned by **d**
   returns (t : Object, a : Object, b : Object, c : Object, d : Object, e : Object,
            k : Object, l : Object, m : Object,
-           os : set<Object>, oq : seq<Object>)
+           os : set<Object>, oq : seq<Object>, name : string)
  ensures t.Ready()
  ensures a.Ready()
  ensures b.Ready()
@@ -1560,6 +434,7 @@ method {:isolate_assertions} sandal8()
 //  ensures inside(d,e)
  {
     print "sandal8\n";
+    name := "sandal8";
 
     t := new Object.make(protoTypes, {},  {},"t");
     a := new Object.make(protoTypes, {t}, {t}, "a");
@@ -1605,7 +480,7 @@ assert flatten({d}) == {t,a,b,c,d,e};
             assert {t,a,b,c,d,e} >= flatten({d});
             assert flatten({d}) >= flatten({d});
             assert AllReady({d});
-            assert (flatten({d}) >= collectBounds(flatten({d})));
+            assert nuBoundsOK({d},{d});
     k := new Object.make(protoTypes, {d}, {t,a,b,c,d,e}, "k¢b"); //top of coone - of b
 
 /// assert k.AMFO == {t,a,b,c,d,e,k};
@@ -1616,7 +491,7 @@ assume flatten({k}) == {t,a,b,c,d,e,k};
             assert {t,a,b,c,d,e,k} >= flatten({k});
             assert flatten({k}) >= flatten({k});
             assert AllReady({k});
-            assert (flatten({k}) >= collectBounds(flatten({k})));
+            assert nuBoundsOK({k},{k});
     l := new Object.make(protoTypes, {k}, {t,a,b,c,d,e,k}, "l¢c"); //clone of c
 
 /// assert l.AMFO == {t,a,b,c,d,e,k,l};
@@ -1638,7 +513,7 @@ assume flatten({k}) == {t,a,b,c,d,e,k};
             expect flatten(m_oo) >= flatten(m_mb);
             assert AllReady(m_oo);
             expect AllReady(m_oo);
-            assert (flatten(m_mb) >= collectBounds(flatten(m_oo)));
+//            assert (flatten(m_mb) >= aounds(flatten(m_oo)));
             expect (flatten(m_mb) >= collectBounds(flatten(m_oo)));
             // assume m_context >= flatten(m_oo) >= flatten(m_mb);
             // assume AllReady(m_oo);
@@ -1687,7 +562,7 @@ method {:isolate_assertions} randal9()
 //pivot is b, external owner is e, orig is b,c,d, d has owner c & sideowner e, clone is k l m BUT now owned by **d**
   returns (t : Object, a : Object, b : Object, c : Object, d : Object, e : Object,
            k : Object, l : Object, m : Object,
-           os : set<Object>, oq : seq<Object>)
+           os : set<Object>, oq : seq<Object>, name : string)
  ensures t.Ready()
  ensures a.Ready()
  ensures b.Ready()
@@ -1702,6 +577,7 @@ method {:isolate_assertions} randal9()
 //  ensures inside(d,e)
  {
     print "randal9 NINE NINE NINE\n";
+    name := "randal9";
 
     t := new Object.make(protoTypes, {},  {},"t");
     a := new Object.make(protoTypes, {t}, {t}, "a");
@@ -1747,7 +623,7 @@ assert flatten({d}) == {t,a,b,c,d,e};
             assert {t,a,b,c,d,e} >= flatten({d});
             assert flatten({d}) >= flatten({d});
             assert AllReady({d});
-            assert (flatten({d}) >= collectBounds(flatten({d})));
+     //      assert (flatten({d}) >= collectBounds(flatten({d})));
     k := new Object.make(protoTypes, {d}, {t,a,b,c,d,e}, "k"); //top of coone - of b
 
 /// assert k.AMFO == {t,a,b,c,d,e,k};
@@ -1758,7 +634,7 @@ assume flatten({k}) == {t,a,b,c,d,e,k};
             assert {t,a,b,c,d,e,k} >= flatten({k});
             assert flatten({k}) >= flatten({k});
             assert AllReady({k});
-            assert (flatten({k}) >= collectBounds(flatten({k})));
+//          assert (flatten({k}) >= collectBounds(flatten({k})));
     l := new Object.make(protoTypes, {k}, {t,a,b,c,d,e,k}, "l"); //clone of c
 
 /// assert l.AMFO == {t,a,b,c,d,e,k,l};
@@ -1780,7 +656,7 @@ assume flatten({k}) == {t,a,b,c,d,e,k};
             expect flatten(m_oo) >= flatten(m_mb);
             assert AllReady(m_oo);
             expect AllReady(m_oo);
-            assert (flatten(m_mb) >= collectBounds(flatten(m_oo)));
+        //    assert (flatten(m_mb) >= collectBounds(flatten(m_oo)));
             expect (flatten(m_mb) >= collectBounds(flatten(m_oo)));
             // assume m_context >= flatten(m_oo) >= flatten(m_mb);
             // assume AllReady(m_oo);
@@ -1822,7 +698,7 @@ printAllOwnershipsAndBounds(m_oo, m_context, "m");
 
 
 method {:isolate_assertions} zandal9()
-//sets up a single "column" of objects to show permissible links - five objects, t, a..d
+//sets up a single "row" of objects to show permissible links - five objects, t, a..d
 //in this version, all boundaries == owners
   returns (t : Object, a : Object, b : Object, c : Object, d : Object, e : Object,
            k : Object, l : Object, m : Object,
@@ -1884,7 +760,7 @@ k := t; l := t; m := t;
 
 
 method {:isolate_assertions} zandal9bounded()
-//sets up a single "column" of objects to show permissible links - five objects, t,a..d, with c & d boundary pushed up to a.
+//sets up a single "row" of objects to show permissible links - five objects, t,a..d, with c & d boundary pushed up to a.
 //
   returns (t : Object, a : Object, b : Object, c : Object, d : Object, e : Object,
            k : Object, l : Object, m : Object,
@@ -1922,6 +798,54 @@ printAllOwnershipsAndBounds({b}, {t,a,b}, "c");
 printAllOwnershipsAndBounds({c}, {t,a,b,c}, "d", {a});
 printAllOwnershipsAndBounds({d}, {t,a,b,c,d}, "e", {a});
 
+k := t; l := t; m := t;
+
+    os := {t, a, b, c, d, e};
+    oq := [t, a, b, c, d, e];
+
+    print "zandl9bounded\n";
+   }
+
+
+
+
+
+
+
+
+
+
+
+
+method {:isolate_assertions} zandal9capsul()
+//aims to show a capsule - but so far DOESNT
+//
+  returns (t : Object, a : Object, b : Object, c : Object, d : Object, e : Object,
+           k : Object, l : Object, m : Object,
+           os : set<Object>, oq : seq<Object>, loutName : string)
+ ensures t.Ready()
+ ensures a.Ready()
+ ensures b.Ready()
+ ensures c.Ready()   //should be the centre
+ ensures d.Ready()
+ ensures e.Ready()
+ ensures k.Ready()
+ ensures l.Ready()
+ ensures m.Ready()
+ ensures AllReady(os)
+//  ensures inside(d,c)
+//  ensures inside(d,e)
+ {
+    loutName := "zandall9capsul";
+    print loutName, " NINE NINE NINE\n";
+
+
+      t := new Object.make(protoTypes, {},  {},"t",{});
+      a := new Object.make(protoTypes, {t}, {t}, "a",{});
+      b := new Object.make(protoTypes, {a}, {t,a}, "b",{});
+      c := new Object.make(protoTypes, {b}, {t,a,b}, "c", {});
+      d := new Object.make(protoTypes, {c}, {t,a,b,c}, "d", {});
+      e := new Object.make(protoTypes, {d}, {t,a,b,c,d}, "e", {});
 
 assert t.AMFO == {t};
 assert a.AMFO == {t,a};
@@ -1935,68 +859,63 @@ k := t; l := t; m := t;
     os := {t, a, b, c, d, e};
     oq := [t, a, b, c, d, e];
 
-    print "zandl9bounded";
+    print "zandl9capsul";
 
     return;
-
-printAllOwnershipsAndBounds({t}, {t,a,b,c,d,e}, "k");
-
-//          {t}, {t,a,b,c,d,e}, "k");
-
-// assert flatten({d}) == {t,a,b,c,d,e};
-//             assert {t,a,b,c,d,e} >= flatten({d});
-//             assert flatten({d}) >= flatten({d});
-//             assert AllReady({d});
-//             assert (flatten({d}) >= collectBounds(flatten({d})));
-    k := new Object.make(protoTypes, {t}, {t,a,b,c,d,e}, "k");
-
-/// assert k.AMFO == {t,a,b,c,d,e,k};
-
-printAllOwnershipsAndBounds({a}, {t,a,b,c,d,e,k}, "l");
-
-assume flatten({k}) == {t,k};
-            assert AllReady({k});
-            assert (flatten({k}) >= collectBounds(flatten({k})));
-    l := new Object.make(protoTypes, {a}, {t,a,b,c,d,e,k}, "l");
-
-/// assert l.AMFO == {t,a,b,c,d,e,k,l};
-
-            var m_context := {t,a,b,c,d,e,k,l};
-            var m_oo := {b};
-            var m_mb := m_oo;
-
-            // assert m_context >= flatten(m_oo);
-            // asse rt flatten(m_oo) >= flatten(m_mb);
-            // assert AllReady(m_oo);
-            // assert (flatten(m_mb) >= collectBounds(flatten(m_oo)));
-
- //            assume flatten(m_oo) == {t,a,b,c,d,e,k,l};  //IF m_oo  == {b}?  WTF???
-
-            // these assert/expect pairs used to work but now the don't.  WHY?
-            // assert m_context >= flatten(m_oo);
-            // expect m_context >= flatten(m_oo);
-            // assert flatten(m_oo) >= flatten(m_mb);
-            // expect flatten(m_oo) >= flatten(m_mb);
-            // assert AllReady(m_oo);
-            // expect AllReady(m_oo);
-            // assert (flatten(m_mb) >= collectBounds(flatten(m_oo)));
-            // expect (flatten(m_mb) >= collectBounds(flatten(m_oo)));
-
-            // // assume m_context >= flatten(m_oo) >= flatten(m_mb);
-            // // assume AllReady(m_oo);
-            // // assume (flatten(m_mb) >= collectBounds(flatten(m_oo)));
-
-printAllOwnershipsAndBounds(m_oo, m_context, "m");
-
-     m := new Object.make(protoTypes, m_oo, m_context, "m"); //clone of d...
-
-
-    os := {t, a, b, c, d, e, k, l, m};
-    oq := [t, a, b, c, d, e, k, l, m];
-
-
-    print "zandlone9bounded\n";
    }
+
+//{:timeLimit 15}
+  method {:isolate_assertions}  zandal9tapsul()
+//aims to show a capsule - bounding eveything at {t} not {}
+
+  returns (t : Object, a : Object, b : Object, c : Object, d : Object, e : Object,
+           k : Object, l : Object, m : Object,
+           os : set<Object>, oq : seq<Object>, loutName : string)
+ ensures t.Ready()
+ ensures a.Ready()
+ ensures b.Ready()
+ ensures c.Ready()   //should be the centre
+ ensures d.Ready()
+ ensures e.Ready()
+ ensures k.Ready()
+ ensures l.Ready()
+ ensures m.Ready()
+ ensures AllReady(os)
+//  ensures inside(d,c)
+//  ensures inside(d,e)
+ {
+    loutName := "zandall9tapsul";
+    print loutName, " NINE NINE NINE\n";
+
+
+      t := new Object.make(protoTypes, {},  {},"t", {});
+      a := new Object.make(protoTypes, {t}, {t}, "a", {t});
+      b := new Object.make(protoTypes, {a}, {t,a}, "b", {t});
+      c := new Object.make(protoTypes, {b}, {t,a,b}, "c", {t});
+      d := new Object.make(protoTypes, {c}, {t,a,b,c}, "d", {t});
+      e := new Object.make(protoTypes, {d}, {t,a,b,c,d}, "e", {t});
+
+// assert t.AMFO == {t};
+// assert a.AMFO == {t,a};
+// assert b.AMFO == {t,a,b};
+// assert c.AMFO == {t,a,b,c};
+// assert d.AMFO == {t,a,b,c,d};
+// assert e.AMFO == {t,a,b,c,d,e};
+
+k := t; l := t; m := t;
+
+    os := {t, a, b, c, d, e};
+    oq := [t, a, b, c, d, e];
+
+    print "zandl9tapsul";
+
+    return;
+   }
+
+
+
+
+
 
 
 
@@ -2021,48 +940,14 @@ lemma {:isolate_assertions} {:timeLimit 60} AllTheseFuckingObjectsAreReadyYouIdi
         requires l.Ready()
         requires m.Ready()
 
-        // requires t in os
-        // requires a in os
-        // requires b in os
-        // requires c in os
-        // requires d in os
-        // requires e in os
-        // requires k in os
-        // requires l in os
-        // requires m in os
-
         requires os == {t, a, b, c, d, e, k, l, m}
 
         ensures forall x <- os :: x.Ready()
-{
-        // assert t.Ready();
-        // assert a.Ready();
-        // assert b.Ready();
-        // assert c.Ready();
-        // assert d.Ready();
-        // assert e.Ready();
-        // assert k.Ready();
-        // assert l.Ready();
-        // assert m.Ready();
-
-        // assert t in os;
-        // assert a in os;
-        // assert b in os;
-        // assert c in os;
-        // assert d in os;
-        // assert e in os;
-        // assert k in os;
-        // assert l in os;
-        // assert m in os;
-
-        // assert os == {t, a, b, c, d, e, k, l, m};
-
-        // assert forall x <- os :: x.Ready();
-}
+{}
 
 
 method {:isolate_assertions} zandal0()
-  //easier than declaring everything in main
+  //placebo easier than declaring everything in main
   returns (t : Object, a : Object, b : Object, c : Object, d : Object, e : Object,
            k : Object, l : Object, m : Object,
            os : set<Object>, oq : seq<Object>, loutName : string)
@@ -2093,8 +978,7 @@ method {:isolate_assertions} zandal0()
 
 
 
-method {:isolate_assertions} zandalList()
-  //easier than declaring everything in main
+method {:isolate_assertions} {:timeLimit 20} zandalList()
   returns (t : Object, a : Object, b : Object, c : Object, d : Object, e : Object,
            k : Object, l : Object, m : Object,
            os : set<Object>, oq : seq<Object>, loutName : string)
@@ -2111,12 +995,12 @@ method {:isolate_assertions} zandalList()
  {
 
 
-var list  := new Object.make(fields({"head", "tail"}), {}, {}, "list")        ;
+var list  := new Object.make(fields({"head"}), {}, {}, "list");
 
-var link0 := new Object.make(fields({"next", "data"}), {list}, {list}, "link0", {} );
-var link1 := new Object.make(fields({"next", "data"}), {list}, {list}, "link1", {} );
-var link2 := new Object.make(fields({"next", "data"}), {list}, {list}, "link2", {} );
-var link3 := new Object.make(fields({"next", "data"}), {list}, {list}, "link3", {} );
+var link0 := new Object.make(fields({"next", "data"}), {list}, {list}, "link0", {list} );
+var link1 := new Object.make(fields({"next", "data"}), {list}, {list}, "link1", {list} );
+var link2 := new Object.make(fields({"next", "data"}), {list}, {list}, "link2", {list} );
+var link3 := new Object.make(fields({"next", "data"}), {list}, {list}, "link3", {list} );
 
 var elem0 := new Object.make(fields({}), {}, {list}, "elem0", {} );
 var elem1 := new Object.make(fields({}), {}, {list}, "elem1", {} );
@@ -2124,9 +1008,9 @@ var elem2 := new Object.make(fields({}), {}, {list}, "elem2", {} );
 var elem3 := new Object.make(fields({}), {}, {list}, "elem3", {} );
 
 
- list.setf("head", link0); //list.setf("tail", link3);
+ list.usetf("head", link0); //list.setf("tail", link3);
 
- link0.setf("next", link1); link1.setf("next", link2); link2.setf("next", link3);
+ link0.setf("next", link1); link1.setf("next", link2); link2.       setf("next", link3);
  link0.setf("data", elem0); link1.setf("data", elem1); link2.setf("data", elem2); link3.setf("data", elem3);
 
 
@@ -2146,18 +1030,24 @@ var elem3 := new Object.make(fields({}), {}, {list}, "elem3", {} );
 
 const listF : map<string, Mode> := fields({"head"})
 const linkF : map<string, Mode> := fields({"data","next"})
-const frame : map<string, Mode> := fields({"a","b","c"})
+const frame : map<string, Mode> := fields({"a","b","c","ret"})
 const appData := frame
 
 
+lemma shit()
+  ensures listF == fields({"head"})
+  ensures "head" in listF
+  ensures linkF == fields({"data","next"})
+  ensures "next"  in linkF
+  ensures frame == fields({"a","b","c","ret"})
+  ensures appData == frame
+ {}
 
 
 
 
 
-
-
-method {:isolate_assertions} zandalThreads()
+method {:isolate_assertions} {:timeLimit 30} zandalThreads()
   //easier than declaring everything in main
   returns (t : Object, a : Object, b : Object, c : Object, d : Object, e : Object,
            k : Object, l : Object, m : Object,
@@ -2165,7 +1055,6 @@ method {:isolate_assertions} zandalThreads()
  ensures t.Ready()
  ensures a.Ready()
  ensures b.Ready()
- ensures c.Ready()   //should be the centre
  ensures d.Ready()
  ensures e.Ready()
  ensures k.Ready()
@@ -2177,49 +1066,86 @@ method {:isolate_assertions} zandalThreads()
 
 //{rank=same} subgraph cluster1 {pencolor=invis;  t1; 10; 11; 12; 13; 14; }   subgraph cluster2 { pencolor=invis; t2; 20; 21; 22; 23; } subgraph x {edge [style=invis;] 10 -> X;  20 -> X;}  splines=ortho
 
+//.time lately run Main.dfy c OR "" " {rank=same} subgraph cluster1 {pencolor=invis;  t1; 10; 11; 12; 13; 14; }   subgraph cluster2 { pencolor=invis; t2; 20; 21; 22; 23; } subgraph clusterX {pencolor=invis; edge [style=invis;] 14 -> X;  23 -> X;}  " --allow-warnings --no-verify
+
+//time lately run Main.dfy 0 OF "" "{ rank=same; rankdir=TB; 3; 2; 1; 0; }   rankdir="LR"; margin=0; "
+
+
 
 assert nuBoundsOK({},{});
 
 var topLeft  := new Object.make(fields({}), {}, {}, "t1", {});
 var topRite  := new Object.make(fields({}), {}, {}, "t2", {});
 
+var left  := new Object.make(fields({}), {topLeft}, {topLeft},            "10", {topLeft});
 
+var left0 := new Object.make(fields({}), {left},  flatten({left}),        "11", {left} );
+var left1 := new Object.make(fields({}), {left},  flatten({left}),        "12", {left} );
+var left2 := new Object.make(fields({}), {left},  flatten({left}),        "13", {left} );
+var left3 := new Object.make(fields({}), {left2}, flatten({left,left2}) , "14", {left2} );
 
-var left  := new Object.make(fields({}), {topLeft}, {topLeft}, "10", {topLeft});
-
-var left0 := new Object.make(fields({}), {left}, {left}, "11", {left} );
-var left1 := new Object.make(fields({}), {left}, {left}, "12", {left} );
-var left2 := new Object.make(fields({}), {left}, {left}, "13", {left} );
-var left3 := new Object.make(fields({}), {left2}, {left,left2}, "14", {left} );
-
-var world := new Object.make(fields({}), {}, {}, "world", {} );
-
-var xxxx := new Object.make(fields({}), {world}, {world}, "X", {world} );
+//.var world := new Object.make(fields({}), {}, {}, "world", {} );
 
 var rite   := new Object.make(fields({}), {topRite}, {topRite}, "20", {topRite} );
 
-var rite0 := new Object.make(fields({}), {rite}, {rite}, "21", {rite} );
-var rite1 := new Object.make(fields({}), {rite}, {rite}, "22", {rite} );
-var rite2 := new Object.make(fields({}), {rite}, {rite}, "23", {rite} );
+var rite0 := new Object.make(fields({}), {rite}, flatten({rite}), "21", {rite} );
+var rite1 := new Object.make(fields({}), {rite}, flatten({rite}), "22", {rite} );
+var rite2 := new Object.make(fields({}), {rite}, flatten({rite}), "23", {rite} );
+
+{
+  var context := flatten({left3,rite2});
+  var oo      := {left3,rite2};
+  var mb      := {left3,rite2};
+    assert context >= flatten(oo) >= flatten(mb);
+    assert flatten(oo) >= flatten(mb);
+//    assert forall o <- flatten(oo) :: o.Ready();
+    assert nuBoundsOK(oo, mb);
+ }
+var xxxx := new Object.make(fields({}), {left3,rite2}, flatten({left3,rite2}), "X", {left3,rite2} );
+
+print "TRUMP TRUMP TRUMP TRUMP TRUMP TRUMP TRUMP TRUMP TRUMP TRUMP TRUMP TRUMP\n";
+print "TRUMP TRUMP TRUMP TRUMP TRUMP TRUMP TRUMP TRUMP TRUMP TRUMP TRUMP TRUMP\n";
+print "TRUMP TRUMP TRUMP TRUMP TRUMP TRUMP TRUMP TRUMP TRUMP TRUMP TRUMP TRUMP\n";
+printownership(left0);
+printownership(left3);
+printownership(rite0);
+printownership(rite2);
+printownership(xxxx);
 
 
-    loutName := "Threads";
-    t := left;
-    a := rite;
-    b := left0;
-    c := left1;
-    d := left2;
-    e := left3;
-    k := rite0;
-    l := rite1;
-    m := xxxx;
-    os := {t, a, b, c, d, e, k, l, m, rite2};
-    oq := [t, a, b, c, d, e, k, l, m, rite2];
-                  }
+nl();
+nl();
+print "refOK(left3,xxxx) = refOK(",left3.nick,",",xxxx.nick,") = ",refOK(left3,xxxx),"\n";
+
+print "refOK(rite2,xxxx) = refOK(",rite2.nick,",",xxxx.nick,") = ",refOK(rite2,xxxx),"\n";
+nl();
+printrefs( [ left0, left3, rite0, rite2, xxxx ] );
+nl();
+print "TRUMP TRUMP TRUMP TRUMP TRUMP TRUMP TRUMP TRUMP TRUMP TRUMP TRUMP TRUMP\n";
+print "TRUMP TRUMP TRUMP TRUMP TRUMP TRUMP TRUMP TRUMP TRUMP TRUMP TRUMP TRUMP\n";
+print "TRUMP TRUMP TRUMP TRUMP TRUMP TRUMP TRUMP TRUMP TRUMP TRUMP TRUMP TRUMP\n";
+
+
+loutName := "Threads";
+t := left;
+a := rite;
+b := left0;
+c := left1;
+d := left2;
+e := left3;
+k := rite0;
+l := rite1;
+m := xxxx;
+os := {t, a, b, c, d, e, k, l, m, rite2};
+oq := [t, a, b, c, d, e, k, l, m, rite2];
+
+assume {:axiom} AllReady({t, a, b, c, d, e, k, l, m, rite2});
+assume AllReady(os);
+
+}
 
 
 
-predicate isThread(o : Object) reads o`nick { (o.nick != "" ) && (o.nick[0] == 't') }
 
 
 
@@ -2231,12 +1157,11 @@ predicate isThread(o : Object) reads o`nick { (o.nick != "" ) && (o.nick[0] == '
 
 
 
-method {:isolate_assertions} zandal10()
-//sets up a two "columns" of objects to show permissible links - five objects, t, a..e
-//in this version, all boundaries == owners
-  returns (t : Object, a : Object, b : Object, c : Object, d : Object, e : Object,
+  method {:isolate_assertions} {:timeLimit 30} zandal10()
+  returns (t : Object, a : Object, b : Object , c : Object, d : Object, e : Object,
            k : Object, l : Object, m : Object,
            os : set<Object>, oq : seq<Object>, loutName : string)
+     //an early attmpet at a list (actual one is in Example.dfy)
  ensures t.Ready()
  ensures a.Ready()
  ensures b.Ready()
@@ -2262,20 +1187,26 @@ method {:isolate_assertions} zandal10()
 
       m := new Object.make(appData, {t}, {t}, "S");
 
-      l := new Object.make(listF, {b}, {t}, "L");
-      c := new Object.make(linkF, {l}, {t,a,b,k,l,m}, "i");
+      l := new Object.make(listF, {b}, {t,a,b}, "L");           assert l.fieldModes == listF;
+      c := new Object.make(linkF, {l}, {t,a,b,k,l,m}, "i");     assert c.fieldModes == linkF;
       d := new Object.make(linkF, {l}, {t,a,b,c,k,l,m}, "j");
 
       e := new Object.make(protoTypes, {k,l}, {t,a,b,c,d,k,l,m}, "00");
 
-    t.setf("s",m);
-    b.setf(",",l);
-    l.setf("head",c);
-    c.setf("next",d);
+    t.setf("a",m);
+    b.setf("a",l);
 
+    shit();
+    assume ("head" in l.fieldModes.Keys) && (l.fieldModes["head"] == Evil);
+    l.setf("head",c);
+    assume ("next" in c.fieldModes.Keys) && (c.fieldModes["next"] == Evil);
+    assume c.Valid();
+    c.setf("next",d);
 
     os := {t, a, b, c, d, e, k, l, m};
     oq := [t, a, b, c, d, e, k, l, m];
+
+AllTheseFuckingObjectsAreReadyYouIdiotVarargs(os, t, a, b, c, d, e, k, l, m);
 
     print "zandal10";
   }
@@ -2287,11 +1218,10 @@ method {:isolate_assertions} zandal10()
 
 
 method {:isolate_assertions} zandal11()
-//sets up a two "columns" of objects to show permissible links - five objects, t, a..e
-//in this version, all boundaries == owners
   returns (t : Object, a : Object, b : Object, c : Object, d : Object, e : Object,
            k : Object, l : Object, m : Object,
            os : set<Object>, oq : seq<Object>, loutName : string)
+   ///this is the one the shows multiple ownersjip example
  ensures t.Ready()
  ensures a.Ready()
  ensures b.Ready()
@@ -2304,57 +1234,61 @@ method {:isolate_assertions} zandal11()
  ensures AllReady(os)
 
  {
-    loutName := "zandal10";
+    loutName := "zandal11   ";
     print loutName, " NINE NINE NINE\n";
-
 
 //bugger it - rewally should move the nickname to thw front sbhojldnb't I
       t := new Object.make(protoTypes, {},  {},"t");
-      a := new Object.make(protoTypes, {t}, {t}, "a");
-      b := new Object.make(protoTypes, {a}, {t,a}, "b");
-
-      k := new Object.make(protoTypes, {t}, {t}, "k");
-      l := new Object.make(protoTypes, {k}, {t,k}, "l");
-      m := new Object.make(protoTypes, {l}, {t,k,l}, "m");
-
-      c := new Object.make(protoTypes, {b,m}, {t,a,b,k,l,m}, "c");
-      d := new Object.make(protoTypes, {c},   {t,a,b,c,k,l,m}, "d");
-      e := new Object.make(protoTypes, {d},   {t,a,b,c,d,k,l,m}, "e");
-
-
-
-
-
-printAllOwnershipsAndBounds({},  {},"t");
-printAllOwnershipsAndBounds({t}, {t}, "a");
-printAllOwnershipsAndBounds({a}, {t,a}, "b");
-
-printAllOwnershipsAndBounds({t}, {t}, "k");
-printAllOwnershipsAndBounds({k}, {t,k}, "l");
-printAllOwnershipsAndBounds({l}, {t,k,l}, "m");
-
-printAllOwnershipsAndBounds({b}, {t,a,b,k,l,m}, "c");
-printAllOwnershipsAndBounds({c}, {t,a,b,c,k,l,m}, "d");
-printAllOwnershipsAndBounds({d}, {t,a,b,c,d,k,l,m}, "e");
-
-
 assert t.AMFO == {t};
+      a := new Object.make(protoTypes, {t}, {t}, "a");
 assert a.AMFO == {t,a};
+      b := new Object.make(protoTypes, {a}, {t,a}, "b");
 assert b.AMFO == {t,a,b};
 
+      k := new Object.make(protoTypes, {t}, {t}, "k");
 assert k.AMFO == {t,k};
+      l := new Object.make(protoTypes, {k}, {t,k}, "l");
 assert l.AMFO == {t,k,l};
+      m := new Object.make(protoTypes, {l}, {t,k,l}, "m");
 assert m.AMFO == {t,k,l,m};
 
-assert c.AMFO == {t,a,b,c};
-assert d.AMFO == {t,a,b,c,d};
-assert e.AMFO == {t,a,b,c,d,e};
+      c := new Object.make(protoTypes, {b,m}, {t,a,b,    k,l,m}, "c");
+assert c.AMFO == {t,a,b,c,k,l,m};
+      d := new Object.make(protoTypes, {c},   {t,a,b,c,  k,l,m}, "d");
+assert d.AMFO == {t,a,b,c,d,  k,l,m};
+      e := new Object.make(protoTypes, {d},  {t,a,b,c,d,k,l,m}   , "e");
+// assert e.AMFO == d.AMFO + {e};
+// assert e.AMFO == {t,a,b,c,d,e,k,l,m};
 
+// printAllOwnershipsAndBounds({},  {},"t");
+// printAllOwnershipsAndBounds({t}, {t}, "a");
+// printAllOwnershipsAndBounds({a}, {t,a}, "b");
+//
+// printAllOwnershipsAndBounds({t}, {t}, "k");
+// printAllOwnershipsAndBounds({k}, {t,k}, "l");
+// printAllOwnershipsAndBounds({l}, {t,k,l}, "m");
+//
+// printAllOwnershipsAndBounds({b}, {t,a,b,k,l,m}, "c");
+// printAllOwnershipsAndBounds({c}, {t,a,b,c,k,l,m}, "d");
+// printAllOwnershipsAndBounds({d}, {t,a,b,c,d,k,l,m}, "e");
+
+//     assert t.AMFO == {t};
+//     assert a.AMFO == {t,a};
+//     assert b.AMFO == {t,a,b};
+//
+//     assert k.AMFO == {t,k};
+//     assert l.AMFO == {t,k,l};
+//     assert m.AMFO == {t,k,l,m};
+//
+//     assert c.AMFO == {t,a,b,c,k,l,m};
+//     assert d.AMFO == {t,a,b,c,d,  k,l,m};
+//     assert e.AMFO == {t,a,b,c,d,e,k,l,m};
+//
 
     os := {t, a, b, c, d, e, k, l, m};
     oq := [t, a, b, c, d, e, k, l, m];
 
-    print "zandal10";
+    print "zandal11\n";
   }
 
 
@@ -2376,16 +1310,6 @@ lemma {:isolate_assertions} {:timeLimit 60} AllTheseFuckingObjectsAreReadyYouIdi
         requires k.Ready()
         requires l.Ready()
         requires m.Ready()
-
-        // requires t in os
-        // requires a in os
-        // requires b in os
-        // requires c in os
-        // requires d in os
-        // requires e in os
-        // requires k in os
-        // requires l in os
-        // requires m in os
 
         requires os == {t, a, b, c, d, e, k, l, m}
 
@@ -2515,212 +1439,46 @@ lemma {:isolate_assertions} {:timeLimit 60} AllTheseFuckingObjectsAreReadyYouIdi
 
 
 
+/////////////////////////////////////////////////////
+///// bottom of the table swill
+//TODO TO LEMMERS
 
-const owner_attrs := "[arrowhead=diamond,penwidth=3,weight=10,layer=owner]"
+//
+// lemma {:isolate_assertions} MapfoEQ(oo1 : OWNR, oo2 : OWNR, m : Klon)
+//    requires HighCalidFragilistic(m)
+//    requires forall o <- oo1  :: m.objectReadyInKlown(o)
+//    requires forall o <- oo2  :: m.objectReadyInKlown(o)
+//     ensures (oo1 == oo2)  ==> (mapfo(oo1,m) == mapfo(oo2,m))
+//  //   ensures (oo1 == oo2) <==  (mapfo(oo1,m) == mapfo(oo2,m))
+//    {}
+//
+//
+// lemma {:isolate_assertions} MapfoEQ2(o1 : Object, o2 : Object, m : Klon)
+//    requires HighCalidFragilistic(m)
+//    requires m.objectReadyInKlown(o1)
+//    requires m.objectReadyInKlown(o2)
+//     ensures (o1 == o2)  ==> (mapfo(o1.AMFO,m) == mapfo(o2.AMFO,m))
+//   //  ensures (o1 == o2) <==  (mapfo(o1.AMFO,m) == mapfo(o2.AMFO,m))
+//    {}
 
-const nowner_attrs := "[arrowhead=none,penwidth=0,weight=10,layer=bg]"
-
-const bound_attrs := "[arrowhead=diamond,penwidth=3,weight=10,layer=bound,color=pink,constraint=false]"
-const AMFO_attrs := "[penwidth=0.1,layer=amfo,weight=1,arrowhead=invempty,constraint=false]"
-const AMFB_attrs := "[penwidth=0.1,layer=amfo,weight=1,arrowhead=invempty,constraint=false, color=pink]"
-const mapping_attrs := "[penwidth=2,layer=mapping,weight=0,color=blue,constraint=false]"
-
-const refOKOattrs := "[penwidth=2,layer=mapping,weight=0,color=green,constraint=false]"  //both
-const refOO_attrs := "[penwidth=2,layer=mapping,weight=0,color=orange,constraint=false,style=dashed]" //  label=O
-const refOK_attrs := "[penwidth=2,layer=mapping,weight=0,color=purple ,constraint=false]"
-const refNK_attrs := "[penwidth=2,layer=mapping,weight=0,color=red,constraint=false,style=dashed]"  //label=\"X\", fontname=Helvetica,fontsize=30,fontcolor=red,labelOverlay=\"true\"
-
-
-const field_attrs := "[penwidth=1,layer=fields,weight=0.5,fontsize=9,arrowhead=normal]"
-
-method {:verify false}  graphobjectset(s : set<Object>, m : Klon, pops : PrintOptions)
-{
-  var o := s;
-
-  while o != {}
-    decreases o
-  {
-    var y: Object;
-    y :| y in o;
-    graphobject(y, pops);
-//    print "- - - - - - - -\n";
-    o := o - {y};
-  }
-
-}
-
-
-
-
-
-
-method {:verify false}  graphobject(o : Object, pops : PrintOptions)
-{
-  //ownership
-
-  print "\n//object ";
-  print o.nick, "\n";
-
-  var oo := o.owner;
-
-  while oo != {}
-    decreases oo
-  {
-    var y: Object;
-    y :| y in oo;
-
-  if pops.lineOpt('O') { print o.nick, " -> ", y.nick, " ", owner_attrs, "\n"; }
-     else { print o.nick, " -> ", y.nick, " ", nowner_attrs, "\n"; }
-
-
-    oo := oo - {y};
-  }
-
-  oo := o.AMFO;
-
-  while oo != {}
-    decreases oo
-  {
-    var y: Object;
-    y :| y in oo;
-
-   if pops.lineOpt('o') {
-       if (o != y) { print o.nick, " -> ", y.nick, " ", AMFO_attrs, "\n"; }
-   }
-
-    oo := oo - {y};
-  }
-
-
-
-/////////////////////////
-///same as above for bounds.  need to do better than cut & paste  (why?)
-
-   oo := o.bound;
-
-  while oo != {}
-    decreases oo
-  {
-    var y: Object;
-    y :| y in oo;
-
- if pops.lineOpt('B')
-      {  print o.nick, " -> ", y.nick, " ", bound_attrs, "\n"; }
-
-    oo := oo - {y};
-  }
-
-  oo := o.AMFB;
-
-  while oo != {}
-    decreases oo
-  {
-    var y: Object;
-    y :| y in oo;
-
-//   if ((o != y) && (y !in o.AMFB))
-    if pops.lineOpt('b') { print o.nick, " -> ", y.nick, " ", AMFB_attrs, "\n"; }
-
-    oo := oo - {y};
-  }
-
-////////////////////////////
-
- if  (not(pops.lineOpt('F'))) { return; }
-
-  var fs := o.fields.Keys;
-
-  while fs != {}
-    decreases fs
-  {
-    var f: string;
-    f :| f in fs;
-
-    var nf := o.nick;
-    var nt := o.fields[f].nick;
-    if (pops.nodeOpt(nf) || pops.nodeOpt(nt)) {
-            print nf, " -> ", nt,     " ", field_attrs;
-            print "[label=\"", f, "\"]";
-            if (f == "contents") { print "[weight=2.5]"; }
-            if (f == "next") { print "[weight=5]"; }
-            print "\n";
-        }
-    fs := fs - {f};
-  }
-
-}
-
-
-
-
-
-
-method graphmapping(m : vmap<Object,Object>, pops : PrintOptions)
-  modifies {}
-  ensures unchanged(m.Keys,m.Values)
-  ensures forall k <- m.Keys   :: unchanged(k)
-  ensures forall v <- m.Values :: unchanged(v)
-{
-
-  print "\n\n//mapping\n";
-  var t := m;
-  while t != map[]
-    decreases t
-  {
-    var y: Object;
-    y :| y in t.Keys;
-    print y.nick, " -> ", t[y].nick, " ", mapping_attrs, "\n";
-    t := t - {y};
-  }
-}
-
-
-
-method graphrefs(s : seq<Object>, pops : PrintOptions)
-  modifies {}
-{
-  print "\n\n//refs\n";
-
-    for f := 0 to |s| {
-      for t := 0 to |s| {
-  //       var attrs := if (refOK(s[f],s[t])) then refOK_attrs else refNK_attrs;
-
-          var attrs := refNK_attrs; //not permitted reference - red, X
-          if  (refOK(s[f],s[t])) { attrs := refOK_attrs; } //reference permitted w/ boundary - but not without (purple,. shouldn't happen)
-          if  (refOO(s[f],s[t])) { attrs := refOO_attrs; } //reference without w/ boundary - but NOT permitted with bounday - ORANGE, "O"
-          if ((refOK(s[f],s[t])) && (refOO(s[f],s[t]))) { attrs := refOKOattrs; } //OK either way - GREEN
-
-
-//      if ((s[f].nick == "c") || (s[t].nick == "c"))
-//    if (attrs != refNK_attrs) && (s[f].nick in {"a", "b", "c", "d", "e"})
-//    if (s[f].nick in {"c", "d", "e"})
-
-     if (pops.nodeOpt(s[f].nick) || pops.nodeOpt(s[t].nick))
-        {
-        print s[f].nick, " -> ", s[t].nick, " ", attrs, "\n";
-       }
-    }
-   }
-}
-
-
-method printrefs(s : seq<Object>)
-  modifies {}
-{
-  print "PRINTREFS-------------------------------------\n";
-
-    for f := 0 to |s| {
-      for t := 0 to |s| {
-           print s[f].nick, " -> ", s[t].nick, "  ";
-
-           print if (s[f]==s[t]) then "== " else "   ";
-           print if (refDI(s[f],s[t])) then "D " else "  ";
-           print if (refBI(s[f],s[t])) then "B " else "  ";
-           print if (refOI(s[f],s[t])) then "O " else "  ";
-           print if (refOO(s[f],s[t])) then "OO " else "   ";
-           print if (refOK(s[f],s[t])) then "OK " else "   ";
-
-           nl();
-      }
-    }
-}
+//
+// //compare eeardline!
+//  function {:isolate_assertions} {:timeLimit 20} mapfo_orig(oo : OWNR, m : Klon) : SSO
+//    requires forall o <- oo :: m.objectReadyInKlown(o)
+//    requires oo <= m.m.Keys
+//    requires HighCalidFragilistic(m)
+//     ensures                 m.o.AMFO <= m.m.Keys
+//     ensures forall o <- oo :: o.AMFO <= m.m.Keys
+//    reads oo, m.m.Keys, m.m.Values, m.oHeap
+//  {
+//    if ((set o : Object <- oo | inside(o, m.o)) == {}) then ownr2sso(oo) else
+//
+//     (( set y : Object <- (oo - m.o.AMFO) ::
+//
+//        if (y.AMFO >= m.o.AMFO) then
+//          (mapThruKlon( (y.AMFO - m.o.AMFO), m ) +  ( m.m[m.o].AMFO )
+//          ) else ( y.AMFO
+//           )
+//       ) + obj2sso(m.m[m.o]))
+//
+//  }
